Heap predicates for Clight states

theories/L7/L6_to_Clight_stack.v
@@ -36,16 +36,18 @@ Require Import
         Lia
         L6.eval L6.algebra L6.Ensembles_util L6.ctx.
 
+Module O := Ptrofs.
+
 Section CODEGEN.
 
-Definition mapi {A B} (f : N -> A -> B) :=
-  fix go (n : N) (xs : list A) : list B :=
+Definition mapi {A B} (f : Z -> A -> B) :=
+  fix go (i : Z) (xs : list A) : list B :=
     match xs with
     | [] => []
-    | x :: xs => f n x :: go (n + 1)%N xs
+    | x :: xs => f i x :: go (i + 1)%Z xs
     end.
 
-(* We only translate hoisted terms *)
+(** We only translate hoisted terms *)
 Definition hoisted_exp := (fundefs * exp)%type.
 Definition make_hoisted_exp (e : exp) : hoisted_exp :=
   match e with
@@ -60,33 +62,33 @@ Definition pretty_fun_name f (nenv : name_env) : string :=
   | None => "not an entry"
   end.
 
-(* The number of parameters to be passed as C function parameters *)
+(** The number of parameters to be passed as C function parameters *)
 Variable (n_param : nat).
 
-(* The size of the args array. No function can take more than max_args parameters. *)
+(** The size of the args array. No function can take more than max_args parameters. *)
 Definition max_args := 1024%Z.
 
-(* fun_env holds mappings
-     f ↦ (|ys|, [0; ..; |ys| - 1]) 
-   for each
-     (Fcons f t ys _ _),
-     (Eletapp _ f _ ys _), or
-     (Eapp f _ ys)
-   in the expression being compiled.
+(** fun_env holds mappings
+      f ↦ (|ys|, [0; ..; |ys| - 1]) 
+    for each
+      (Fcons f t ys _ _),
+      (Eletapp _ f _ ys _), or
+      (Eapp f _ ys)
+    in the expression being compiled.
 
-   The list [0; ..; |ys| - 1] gives the locations of f's arguments in the args array.
-   (Simple for now, but may get fancier with custom calling conventions) *)
+    The list [0; ..; |ys| - 1] gives the locations of f's arguments in the args array.
+    (Simple for now, but may get fancier with custom calling conventions) *)
 Fixpoint compute_fun_env' (fenv : fun_env) (e : exp) : fun_env :=
   match e with
   | Econstr x t ys e' => compute_fun_env' fenv e'
   | Ecase x cs => fold_left (fun fenv '(_, e) => compute_fun_env' fenv e) cs fenv
   | Eproj x t n v e' => compute_fun_env' fenv e'
   | Eletapp x f t ys e' =>
-    compute_fun_env' (M.set f (N.of_nat (length ys), mapi (fun n _ => n) 0 ys) fenv) e'
+    compute_fun_env' (M.set f (N.of_nat (length ys), mapi (fun n _ => Z.to_N n) 0 ys) fenv) e'
   | Efun fds e' =>
     let fenv := compute_fun_env_fundefs fds fenv in
     compute_fun_env' fenv e'
-  | Eapp f t ys => M.set f (N.of_nat (length ys), mapi (fun n _ => n) 0 ys) fenv
+  | Eapp f t ys => M.set f (N.of_nat (length ys), mapi (fun n _ => Z.to_N n) 0 ys) fenv
   | Eprim x p ys e' => compute_fun_env' fenv e'
   | Ehalt x => fenv
   end
@@ -94,15 +96,15 @@ with compute_fun_env_fundefs fds fenv : fun_env :=
   match fds with
   | Fnil => fenv
   | Fcons f t ys e fds' =>
-    let fenv := M.set f (N.of_nat (length ys), mapi (fun n _ => n) 0 ys) fenv in
+    let fenv := M.set f (N.of_nat (length ys), mapi (fun n _ => Z.to_N n) 0 ys) fenv in
     let fenv := compute_fun_env' fenv e in
     compute_fun_env_fundefs fds' fenv
   end.
 Definition compute_fun_env : hoisted_exp -> fun_env :=
   fun '(fds, e) => compute_fun_env' (M.empty _) (Efun fds e).
 
-(* Max number of words allocated by e up to the next function call.
-   (Only compute up to next function call because that's when GC will run next) *)
+(** Max number of words allocated by e up to the next function call.
+    (Only compute up to next function call because that's when GC will run next) *)
 Fixpoint max_allocs (e : exp) : nat :=
   match e with
   | Econstr x t vs e' =>
@@ -123,9 +125,9 @@ Fixpoint max_allocs (e : exp) : nat :=
 
 (** * Clight abbreviations *)
 
-(* typedef intnat value; (See values.h, config.h)
+(** typedef intnat value; (See values.h, config.h)
 
-   NOTE: in Clight, SIZEOF_PTR == SIZEOF_INT *)
+    NOTE: in Clight, SIZEOF_PTR == SIZEOF_INT *)
 Definition value :=
   if Archi.ptr64
   then Tlong Signed noattr
@@ -137,32 +139,32 @@ Definition make_cint (z : Z) (t : type) : expr :=
   then Econst_long (Int64.repr z) t
   else Econst_int (Int.repr z) t.
 
-(* struct thread_info {
-     value *alloc;
-     value *limit;
-     struct heap *heap;
-     value args[MAX_ARGS];
-     struct stack_frame *fp;
-     uintnat nalloc;
-   };
+(** struct thread_info {
+      value *alloc;
+      value *limit;
+      struct heap *heap;
+      value args[MAX_ARGS];
+      struct stack_frame *fp;
+      uintnat nalloc;
+    };
 
-   Zoe: nalloc is the number of allocations until the next GC call so that GC can perform a test. 
-   Note that it will be coerced to UL from ULL. That should be safe for the values we're using but 
-   consider changing it too. *)
+    Zoe: nalloc is the number of allocations until the next GC call so that GC can perform a test. 
+    Note that it will be coerced to UL from ULL. That should be safe for the values we're using but 
+    consider changing it too. *)
 Context (thread_info_id alloc_id limit_id heap_id args_id fp_id nalloc_id : ident).
 Notation threadStructInf := (Tstruct thread_info_id noattr). 
 Notation threadInf := (Tpointer threadStructInf noattr).
 (* TODO: snake-case-ify; currently used by glue code generator *)
 
-(* struct stack_frame {
-     value *next;
-     value *root;
-     struct stack_frame *prev;
-   }; *)
+(** struct stack_frame {
+      value *next;
+      value *root;
+      struct stack_frame *prev;
+    }; *)
 Context (stack_frame_id next_fld root_fld prev_fld : ident).
 Notation stack_frame := (Tstruct stack_frame_id noattr).
 
-(* Declarations for the above structs, in abstract syntax *)
+(** Declarations for the above structs, in abstract syntax *)
 Definition composites : list composite_definition :=
   Composite stack_frame_id Struct
             ((next_fld, tptr value) ::
@@ -181,7 +183,7 @@ Definition composites : list composite_definition :=
             noattr ::
    nil.
 
-(* Each generated function takes a (struct thread_info *tinfo) as argument *)
+(** Each generated function takes a (struct thread_info *tinfo) as argument *)
 Context (tinfo_id : ident).
 Definition tinfo := Etempvar tinfo_id threadInf.
 Definition tinfd := Ederef tinfo threadStructInf.
@@ -191,10 +193,10 @@ Notation "tinfo->args" := (Efield tinfd args_id (Tarray value max_args noattr)).
 Notation "tinfo->fp" := (Efield tinfd fp_id (tptr stack_frame)).
 Notation "tinfo->nalloc" := (Efield tinfd nalloc_id value).
 
-(* Each generated function body declares the following local variables:
-     struct stack_frame frame;
-     value roots[size];
-   where size upper bounds the number of variables live at GC calls. *)
+(** Each generated function body declares the following local variables:
+      struct stack_frame frame;
+      value roots[size];
+    where size upper bounds the number of variables live at GC calls. *)
 Context (frame_id roots_id : ident).
 Definition roots_ty size := Tarray value size noattr.
 Definition roots := Etempvar roots_id (tptr value).
@@ -206,30 +208,32 @@ Definition stack_decl size : list (ident * type) :=
   (frame_id, stack_frame) ::
   (roots_id, roots_ty size) :: nil.
 
-(* Each generated function body also declares the following local variables:
-     value *alloc;
-     value *limit; *)
+(** Each generated function body also declares the following local variables:
+      value *alloc;
+      value *limit; *)
 Definition alloc := Etempvar alloc_id (tptr value).
 Definition limit := Etempvar limit_id (tptr value).
 
 (* Variable (isptr_id : ident). (* ident for the is_ptr external function *) *)
 
-(* void garbage_collect(struct thread_info *tinfo);
-   struct thread_info *make_tinfo(void);
-   value *export(struct thread_info *ti); *)
+(** void garbage_collect(struct thread_info *tinfo);
+    struct thread_info *make_tinfo(void);
+    value *export(struct thread_info *ti); *)
 Variable (gc_id : ident).
 Definition gc := Evar gc_id (Tfunction (Tcons threadInf Tnil) Tvoid cc_default).
 Definition make_tinfo_ty := Tfunction Tnil threadInf cc_default.
 Definition export_ty := Tfunction (Tcons threadInf Tnil) (tptr value) cc_default.
 Variable (body_id : ident).
 
+(** void __builtin_unreachable(void);
+    For marking the default cases of switch blocks as unreachable. *)
 Variable (builtin_unreachable_id : ident).
 Definition builtin_unreachable : statement :=
   let f := Evar builtin_unreachable_id (Tfunction Tnil Tvoid cc_default) in
   Scall None f nil.
 
-(* fun_ty n = void(struct thread_info *ti, value, .. min(n_param, n) times)
-   prim_ty n = value(value, .. n times) *)
+(** fun_ty n = void(struct thread_info *ti, value, .. min(n_param, n) times)
+    prim_ty n = value(value, .. n times) *)
 Definition value_tys (n : nat) : typelist := Nat.iter n (Tcons value) Tnil.
 Definition fun_ty (n : nat) := Tfunction (Tcons threadInf (value_tys (min n_param n))) Tvoid cc_default.
 Definition prim_ty (n : nat) := Tfunction (value_tys n) value cc_default.
@@ -258,9 +262,9 @@ Variable (cenv : ctor_env).
 Variable (fenv : fun_env).
 
 Inductive ctor_rep : Type :=
-(* [enum t] represents a constructor with no parameters with ordinal [t] *)
+(** [enum t] represents a constructor with no parameters with ordinal [t] *)
 | enum : N -> ctor_rep
-(* [boxed t a] represents a construct with arity [a] and ordinal [t]  *)
+(** [boxed t a] represents a construct with arity [a] and ordinal [t]  *)
 | boxed : N -> N -> ctor_rep.
 
 Definition get_ctor_rep (c : ctor_tag) : error ctor_rep :=
@@ -281,22 +285,20 @@ Definition make_tag (r : ctor_rep) : expr :=
   | boxed t a => c_int (rep_boxed t a) value
   end%Z.
 
-(* To use variables in Clight expressions, need variable name and its type.
-   Variables that refer to functions must have type
-     void(struct thread_info *ti, val, ..)
-                                  ------- n times
-   where n = min(n_param, arity of the function).
+(** To use variables in Clight expressions, need variable name and its type.
+    Variables that refer to functions must have type
+      void(struct thread_info *ti, val, ..)
+                                   ------- n times
+    where n = min(n_param, arity of the function).
 
-   All other variables just have type val. 
+    All other variables just have type val. 
 
-   make_var x =
-     Ecast (Evar x suitable-fn-type) value if x is a toplevel function
-     Etempvar x value otherwise *)
+    make_var x =
+      Ecast (Evar x suitable-fn-type) value if x is a toplevel function
+      Etempvar x value otherwise *)
 Definition make_var (x : ident) :=
   match M.get x fenv with
-  (* if f is a function with arity |locs|, then x has function type *)
   | Some (_, locs) => Ecast (Evar x (fun_ty (length locs))) value
-  (* otherwise, x is just a regular variable *)
   | None => var x
   end.
 
@@ -346,8 +348,8 @@ Definition make_cases (translate_body : exp -> error (statement * FVSet * N)) :=
       end
     end.
 
-(* Use limit and alloc to check whether the nursery contains n words of free space.
-   If not, invoke GC. *)
+(** Use limit and alloc to check whether the nursery contains n words of free space.
+    If not, invoke GC. *)
 Definition create_space (n : nat) : statement :=
   let n := c_int (Z.of_nat n) value in 
   Sifthenelse
@@ -360,24 +362,24 @@ Definition create_space (n : nat) : statement :=
      limit_id ::= tinfo->limit)
     Sskip.
 
-(* fvs ∪ ({x} ∩ locals) *)
+(** fvs ∪ ({x} ∩ locals) *)
 Definition add_local_fv fvs x := if PS.mem x locals then PS.add x fvs else fvs.
 Definition add_local_fvs fvs xs := fold_left add_local_fv xs fvs.
 
-(* Returns (C code for e, FV(e) ∩ locals, number of stack slots needed) 
-   Number of stack slots needed = 
-     max(|FV(e')∩locals| for each Eletapp x f t ys e' we encounter in e) *)
+(** Returns (C code for e, FV(e) ∩ locals, number of stack slots needed) 
+    Number of stack slots needed = 
+      max(|FV(e')∩locals| for each Eletapp x f t ys e' we encounter in e) *)
 Fixpoint translate_body (e : exp) {struct e} : error (statement * FVSet * N) :=
   match e with
-  (* [[let x = Con c ys in e]] =
-       if c is unboxed (and ys = []),
-         x = (c<<1) + 1;
-       if x is boxed,
-         x = alloc + 1;
-         alloc += 1 + |ys|;
-         x[-1] = |ys|<<10 + c; (assume |ys|<256)
-         x[0 .. |ys| - 1] = ys;
-       [[e]] *)
+  (** [[let x = Con c ys in e]] =
+        if c is unboxed (and ys = []),
+          x = (c<<1) + 1;
+        if x is boxed,
+          x = alloc + 1;
+          alloc += 1 + |ys|;
+          x[-1] = |ys|<<10 + c; (assume |ys|<256)
+          x[0 .. |ys| - 1] = ys;
+        [[e]] *)
   | Econstr x c ys e =>
     rep <- get_ctor_rep c ;;
     stm_constr <-
@@ -387,13 +389,13 @@ Fixpoint translate_body (e : exp) {struct e} : error (statement * FVSet * N) :=
         ret (x ::= Ecast (alloc +' c_int 1 value) value;
              alloc_id ::= alloc +' c_int (Z.of_N (a + 1)) value;
              (var x).[-1] :::= make_tag rep;
-             statements (mapi (fun n y => (var x).[Z.of_N n] :::= make_var y) 0 ys))
+             statements (mapi (fun i y => (var x).[i] :::= make_var y) 0 ys))
       end ;;
     '(stm_e, fvs_e, n_e) <- translate_body e ;;
     ret ((stm_constr; stm_e), add_local_fvs (PS.remove x fvs_e) ys, n_e)
-  (* [[Ecase x cs]] = 
-       if (isptr(x)) { switch on x[-1]&255 over boxed cases } 
-       else { switch on x>>1 over unboxed cases } *)
+  (** [[Ecase x cs]] = 
+        if (isptr(x)) { switch on x[-1]&255 over boxed cases } 
+        else { switch on x>>1 over unboxed cases } *)
   | Ecase x cs =>
     '(boxed_cases, unboxed_cases, fvs_cs, n_cs) <- make_cases translate_body cs ;;
     ret (Sifthenelse
@@ -401,27 +403,27 @@ Fixpoint translate_body (e : exp) {struct e} : error (statement * FVSet * N) :=
           (Sswitch ((var x).[-1] &' make_cint 255 value) boxed_cases)
           (Sswitch (var x >>' make_cint 1 value) unboxed_cases),
          add_local_fv fvs_cs x, n_cs)
-  (* [[let x = f(y, ..) in e]] =
-       push local variables live after call (= locals∩(FV(e)\x)) onto frame
-       push frame onto shadow stack
-       call f (may GC)
-       x = args[1]
-       if max_allocs(e) > 0,
-         if x is live after the call (<-> x ∈ locals∩FV(e)), push it onto frame
-         use GC to create max_allocs(e) words of free space on the heap
-         if x was pushed, pop x out of frame (in case it was moved by GC)
-       pop locals out of frame (in case they were moved by GC)
-       pop frame from shadow stack
-       [[e]] *)
+  (** [[let x = f(y, ..) in e]] =
+        push local variables live after call (= locals∩(FV(e)\x)) onto frame
+        push frame onto shadow stack
+        call f (may GC)
+        x = args[1]
+        if max_allocs(e) > 0,
+          if x is live after the call (<-> x ∈ locals∩FV(e)), push it onto frame
+          use GC to create max_allocs(e) words of free space on the heap
+          if x was pushed, pop x out of frame (in case it was moved by GC)
+        pop locals out of frame (in case they were moved by GC)
+        pop frame from shadow stack
+        [[e]] *)
   | Eletapp x f t ys e =>
     '(stm_e, live_after_call, n_e) <- translate_body e ;;
     let live_minus_x := PS.remove x live_after_call in
     let live_minus_x_list := PS.elements live_minus_x in
     let n_live_minus_x := Z.of_nat (length live_minus_x_list) in
     call <- make_fun_call false f ys ;;
-    let retrieve_roots xs := statements (mapi (fun n x => x ::= roots.[Z.of_N n]) 0 xs) in
+    let retrieve_roots xs := statements (mapi (fun i x => x ::= roots.[i]) 0 xs) in
     let stm :=
-      statements (mapi (fun n x => roots.[Z.of_N n] :::= var x) 0 live_minus_x_list);
+      statements (mapi (fun i x => roots.[i] :::= var x) 0 live_minus_x_list);
       frame.next :::= roots +' c_int n_live_minus_x value;
       tinfo->fp :::= &frame;
       call;
@@ -441,22 +443,22 @@ Fixpoint translate_body (e : exp) {struct e} : error (statement * FVSet * N) :=
     in
     ret (stm, add_local_fvs live_minus_x (f :: ys),
          N.max n_e (N.of_nat (PS.cardinal live_after_call)))
-  (* [[let x = y.n in e]] = (x = y[n]; [[e]]) *)
+  (** [[let x = y.n in e]] = (x = y[n]; [[e]]) *)
   | Eproj x t n y e =>
     '(stm_e, fvs_e, n_e) <- translate_body e ;;
     ret ((x ::= (var y).[Z.of_N n]; stm_e), add_local_fv (PS.remove x fvs_e) y, n_e)
   | Efun fnd e => Err "translate_body: nested function detected"
-  (* [[f(ys)]] = call f *)
+  (** [[f(ys)]] = call f *)
   | Eapp f t ys =>
     call <- make_fun_call true f ys ;;
     ret (call, add_local_fvs PS.empty (f :: ys), 0)%N
-  (* [[let x = p(ys) in e]] = (x = p(ys); [[e]]) *)
+  (** [[let x = p(ys) in e]] = (x = p(ys); [[e]]) *)
   | Eprim x p ys e =>    
     '(stm_e, fvs_e, n_e) <- translate_body e ;;
     ret ((Scall (Some x) (Evar p (prim_ty (length ys))) (map make_var ys);
           stm_e),
          add_local_fvs (PS.remove x fvs_e) ys, n_e)
-  (* [[halt x]] = (args[1] = x; store alloc and limit in tinfo) *)
+  (** [[halt x]] = (args[1] = x; store alloc and limit in tinfo) *)
   | Ehalt x =>
     ret ((tinfo->args.[1] :::= make_var x;
           tinfo->alloc :::= alloc;
@@ -490,22 +492,22 @@ Fixpoint translate_fundefs (fds : fundefs) (nenv : name_env) : error (list defin
     match M.get f fenv with
     | None => Err "translate_fundefs: Unknown function name"
     | Some (_, locs) =>
-      (* [[f(xs.., ys..) = e]] (where |xs| = n_param) =
-           void f(thread struct_info *tinfo, value x, ..) {
-             alloc = tinfo->alloc;
-             limit = tinfo->limit;
-             args = tinfo->args;
-             For n_param <= i < |xs|+|ys|,
-               y_i = args[locs_i];
-             initialize shadow stack frame
-             if max_allocs(e) > 0,
-               push locals live in e onto frame
-               push frame onto shadow stack
-               use GC to create max_allocs(e) words of free space on the heap
-               pop locals out of frame
-               pop frame from shadow stack
-             [[e]]
-           } *)
+      (** [[f(xs.., ys..) = e]] (where |xs| = n_param) =
+            void f(thread struct_info *tinfo, value x, ..) {
+              alloc = tinfo->alloc;
+              limit = tinfo->limit;
+              args = tinfo->args;
+              For n_param <= i < |xs|+|ys|,
+                y_i = args[locs_i];
+              initialize shadow stack frame
+              if max_allocs(e) > 0,
+                push locals live in e onto frame
+                push frame onto shadow stack
+                use GC to create max_allocs(e) words of free space on the heap
+                pop locals out of frame
+                pop frame from shadow stack
+              [[e]]
+            } *)
       let locals := PS.elements (exp_bv e) in
       let xs_set := union_list PS.empty xs in
       '(body, live_xs, stack_slots) <- translate_body (union_list xs_set locals) nenv e ;;
@@ -519,11 +521,11 @@ Fixpoint translate_fundefs (fds : fundefs) (nenv : name_env) : error (list defin
         statements (map (fun '(x, i) => x ::= tinfo->args.[Z.of_N i]) (skipn n_param (combine xs locs)));
         init_shadow_stack_frame;
         match allocs with 0 => Sskip | S _ as allocs =>
-          statements (mapi (fun n x => roots.[Z.of_N n] :::= var x) 0 live_xs_list);
+          statements (mapi (fun i x => roots.[i] :::= var x) 0 live_xs_list);
           frame.next :::= roots +' c_int (Z.of_N n_live_xs) value;
           tinfo->fp :::= &frame;
           create_space allocs;
-          statements (mapi (fun n x => x ::= roots.[Z.of_N n]) 0 live_xs_list);
+          statements (mapi (fun i x => x ::= roots.[i]) 0 live_xs_list);
           tinfo->fp :::= frame.prev
         end;
         body
@@ -538,19 +540,19 @@ Fixpoint translate_fundefs (fds : fundefs) (nenv : name_env) : error (list defin
     end
   end.
 
-(* [[let rec fds in e]] =
-     [[fds]]
-     value body(struct thread_info *tinfo) {
-       alloc = tinfo->alloc;
-       limit = tinfo->limit;
-       args = tinfo->args;
-       initialize shadow stack frame
-       if max_allocs(e) > 0,
-         use GC to create max_allocs(e) words of free space on the heap
-         (no need to push or pop locals because nothing is live yet)
-       [[e]]
-       return tinfo->args[1];
-     } *)
+(** [[let rec fds in e]] =
+      [[fds]]
+      value body(struct thread_info *tinfo) {
+        alloc = tinfo->alloc;
+        limit = tinfo->limit;
+        args = tinfo->args;
+        initialize shadow stack frame
+        if max_allocs(e) > 0,
+          use GC to create max_allocs(e) words of free space on the heap
+          (no need to push or pop locals because nothing is live yet)
+        [[e]]
+        return tinfo->args[1];
+      } *)
 Definition translate_program (fds_e : hoisted_exp) (nenv : name_env) : error (list definition) :=
   let '(fds, e) := fds_e in
   let locals := PS.elements (exp_bv e) in
@@ -744,452 +746,80 @@ Definition compile e cenv nenv : error (name_env * Clight.program * Clight.progr
 
 Section PROOF.
 
+Definition get_ith {A} := @Coqlib.list_nth_z A.
+
+Fixpoint set_ith {A} (xs : list A) (i : Z) (y : A) : list A :=
+  match xs with
+  | [] => []
+  | x :: xs => if Z.eq_dec i 0 then y :: xs else x :: set_ith xs (Z.pred i) y
+  end.
+
+Lemma get_ith_range {A} (xs : list A) i y :
+  get_ith xs i = Some y ->
+  (0 <= i < Z.of_nat (length xs))%Z.
+Proof.
+  revert i; induction xs as [|x xs IHxs]; [easy|intros* Hget].
+  cbn in Hget; destruct (Coqlib.zeq i 0) as [|Hne]; [subst|];
+  change (length (x :: xs)) with (S (length xs)); [lia|].
+  specialize (IHxs (Z.pred i) Hget); lia.
+Qed.
+
+Lemma set_ith_cons {A} (x : A) xs i y :
+  set_ith (x :: xs) i y = if Z.eq_dec i 0 then y :: xs else x :: set_ith xs (Z.pred i) y.
+Proof. reflexivity. Qed.
+
+Lemma set_ith_len {A} (y : A) xs i :
+  length (set_ith xs i y) = length xs.
+Proof.
+  revert i; induction xs as [|x xs IHxs]; [auto|intros i; cbn].
+  destruct (Z.eq_dec i 0) as [|Hne]; [now subst|now cbn].
+Qed.
+
+Lemma get_ith_in_range {A} (xs : list A) i :
+  (0 <= i < Z.of_nat (length xs))%Z ->
+  exists x, get_ith xs i = Some x.
+Proof.
+  revert i; induction xs as [|x xs IHxs]; [cbn; lia|intros i Hi].
+  cbn in *; destruct (Coqlib.zeq i 0); [eexists; reflexivity|apply IHxs; lia].
+Qed.
+
+Lemma ith_gss {A} (xs : list A) i y :
+  (0 <= i < Z.of_nat (length xs))%Z ->
+  get_ith (set_ith xs i y) i = Some y.
+Proof.
+  revert i; induction xs as [|x xs IHxs]; [cbn; lia|intros i Hi].
+  cbn; destruct (Z.eq_dec i 0) as [Heq|Hne]; [now subst|].
+  cbn in *; destruct (Coqlib.zeq i 0); [easy|apply IHxs; lia].
+Qed.
+
+Lemma ith_gso {A} (xs : list A) i j y :
+  i <> j ->
+  get_ith (set_ith xs i y) j = get_ith xs j.
+Proof.
+  revert i j; induction xs as [|x xs IHxs]; [easy|intros i j Hne].
+  cbn; destruct (Z.eq_dec i 0); [subst|].
+  - cbn; now destruct (Coqlib.zeq j 0).
+  - cbn; destruct (Coqlib.zeq j 0); [easy|now rewrite IHxs].
+Qed.
+
+Definition All := fold_right and True.
+Definition Ex := fold_right or False.
+Definition Bigcup {A} := fold_right (Union _) (Empty_set A).
+
+Lemma All_app xs ys : All (xs ++ ys) <-> All xs /\ All ys. Proof. induction xs; cbn; tauto. Qed.
+Lemma All_cons x xs : All (x :: xs) <-> x /\ All xs. Proof. reflexivity. Qed.
+
+Ltac sets := eauto with Ensembles_DB Decidable_DB.
+
+Lemma Bigcup_app {A} xs ys : @Bigcup A (xs ++ ys) <--> Bigcup xs :|: Bigcup ys.
+Proof. induction xs; cbn; [sets|]. rewrite IHxs; sets. Qed.
+Lemma Bigcup_cons {A} x xs : @Bigcup A (x :: xs) <--> x :|: Bigcup xs. Proof. reflexivity. Qed.
+
 Variable (pr : prims).
 Variable (cenv : ctor_env).
 Variable (fenv : fun_env).
 
-(* The C program produced by the code generator *)
-Variable (prog : program).
-
-(* Its global environment *)
-Let prog_genv : genv := globalenv prog.
-
-Definition make_vint (z : Z) : Values.val :=
-  if Archi.ptr64
-  then Vlong (Int64.repr z)
-  else Values.Vint (Int.repr z).
-
-Fixpoint closed_val (v : cps.val) :=
-  match v with
-  | Vconstr c vs => fold_right (fun v P => closed_val v /\ P) True vs
-  | Vfun ρ fds f => M.bempty ρ = true
-  | Vint _ => True
-  end.
-
-Definition int_chunk := if Archi.ptr64 then Mint64 else Mint32.
-Definition int_size := size_chunk int_chunk.
-Definition header_offset o := Ptrofs.unsigned (Ptrofs.sub o (Ptrofs.repr int_size)).
-Definition index_offset o i := Ptrofs.unsigned (Ptrofs.add o (Ptrofs.repr (int_size * i))).
-
-(** * Tools for reasoning about Clight *)
-
-(* Bigstep evaluation of statements: unlike exec_stmt,
-   - Force the trace to be empty
-   - Force outcome to be Out_normal (i.e., statement can't exit early
-     via return/break/continue) *)
-Definition texec := fun '(env, tenv, m, stmt) '(tenv', m') =>
-  exec_stmt prog_genv env tenv m stmt Events.E0 tenv' m' Out_normal.
-Infix "⇓" := texec (at level 80, no associativity).
-
-(* Similar notations for bigstep evaluation of l- and r-values *)
-Definition eval_expr_operator := fun '(env, tenv, m, e) v =>
-  eval_expr prog_genv env tenv m e v.
-Definition eval_lvalue_operator := fun '(env, tenv, m, e) '(b, o) =>
-  eval_lvalue prog_genv env tenv m e b o.
-Infix "⇓ᵣ" := eval_expr_operator (at level 80).
-Infix "⇓ₗ" := eval_lvalue_operator (at level 80).
-
-(** ** "Reductions" in machine state *)
-
-(* (env1, tenv1, m1, stmt1) "reduces to" (env2, tenv2, m2, stmt2) if every terminating
-   execution starting from (env2, tenv2, m2, stmt2) can be used to construct an execution
-   starting from (env1, tenv1, m1, stmt1) *)
-Definition Clight_state_red := fun '(env1, tenv1, m1, stmt1) '(env2, tenv2, m2, stmt2) =>
-  forall tenv' m',
-  (env2, tenv2, m2, stmt2) ⇓ (tenv', m') ->
-  (env1, tenv1, m1, stmt1) ⇓ (tenv', m').
-Infix "-->" := Clight_state_red (at level 80).
-
-Lemma Cred_trans s1 s2 s3 :
-  s1 --> s2 -> s2 --> s3 -> s1 --> s3.
-Proof. destruct s1 as [[[??]?]?], s2 as [[[??]?]?], s3 as [[[??]?]?]; cbn; eauto. Qed.
-
-Lemma Cred_seq_assoc s1 s2 s3 env tenv m :
-  (env, tenv, m, ((s1; s2); s3)) --> (env, tenv, m, (s1; (s2; s3))).
-Proof.
-  intros tenv' m' Hs123; inv Hs123; [|contradiction].
-  inv H9; [|contradiction].
-  unfold "⇓"; rewrite <- H4, <- Events.Eapp_assoc; repeat (eapply exec_Sseq_1; eauto).
-Qed.
-
-Lemma Cred_skip env tenv m s :
-  (env, tenv, m, (Sskip; s)) --> (env, tenv, m, s).
-Proof.
-  intros tenv' m' Hexec.
-  unfold "⇓"; change Events.E0 with (Events.Eapp Events.E0 Events.E0).
-  eapply exec_Sseq_1; [constructor|eauto].
-Qed.
-
-Lemma Cred_set env tenv m x a v s :
-  (env, tenv, m, a) ⇓ᵣ v ->
-  (env, tenv, m, (x ::= a; s)) --> (env, M.set x v tenv, m, s).
-Proof.
-  intros Heval tenv' m' Hexec.
-  unfold "⇓"; change Events.E0 with (Events.Eapp Events.E0 Events.E0).
-  eapply exec_Sseq_1; [now constructor|eauto].
-Qed.
-
-Lemma Cred_assign env tenv m a1 a2 v_pre v b o m' s :
-  (env, tenv, m, a1) ⇓ₗ (b, o) ->
-  (env, tenv, m, a2) ⇓ᵣ v_pre ->
-  sem_cast v_pre (typeof a2) (typeof a1) m = Some v ->
-  assign_loc prog_genv (typeof a1) m b o v m' ->
-  (env, tenv, m, (a1 :::= a2; s)) --> (env, tenv, m', s).
-Proof.
-  intros Heval_dst Heval_src Hcast Hassign tenv' m'' Hexec.
-  unfold "⇓"; change Events.E0 with (Events.Eapp Events.E0 Events.E0).
-  eapply exec_Sseq_1; [now econstructor|eauto].
-Qed.
-
-Lemma Cred_if env tenv m a v b s1 s2 s :
-  (env, tenv, m, a) ⇓ᵣ v ->
-  bool_val v (typeof a) m = Some b ->
-  (env, tenv, m, (Sifthenelse a s1 s2; s)) -->
-  (env, tenv, m, ((if b then s1 else s2); s)).
-Proof.
-  intros Heval Hbool tenv' m' Hexec.
-  unfold "⇓" in *; inv Hexec; [|easy].
-  eapply exec_Sseq_1; [econstructor|]; eauto.
-Qed.
-
-Lemma Cred_if' env tenv m a v b s1 s2 :
-  (env, tenv, m, a) ⇓ᵣ v ->
-  bool_val v (typeof a) m = Some b ->
-  (env, tenv, m, Sifthenelse a s1 s2) -->
-  (env, tenv, m, if b then s1 else s2).
-Proof. intros Heval Hbool tenv' m' Hexec; econstructor; eauto. Qed.
-
-(** ** Address spaces *)
-
-Definition addrs := Ensemble (block * Z).
-Definition Addrs m : addrs := fun '(b, o) => exists chunk v, Mem.load chunk m b o = Some v.
-
-(** * Logical relation between λ-ANF and Clight *)
-
-Notation "'match!' e1 'with' p 'in' e2" :=
-  (match e1 with p => e2 | _ => False end)
-  (at level 80, p pattern, e1 at next level, right associativity).
-
-Context {fuel : Type} {Hf : @fuel_resource fuel} {trace : Type} {Ht : @trace_resource trace}.
-
-(* Bigstep evaluation of L6 terms *)
-Definition bstep_res := fun '(ρ, e, cin) '(v, cout) =>
-  bstep_fuel cenv ρ e cin (Res v) cout.
-Infix "⇓cps" := bstep_res (at level 80).
-
-Section CycleBreakers.
-
-Context (rel_val : forall (k : nat) (v : cps.val) (m : Memory.mem) (cv : Values.val), Prop).
-
-Definition rel_exp' k (ρ : env) (e : cps.exp) env tenv m stmt : Prop :=
-  forall v (cin : fuel) (cout : trace),
-  (* if running e in environment ρ yields a value v in j <= k cost, *)
-  to_nat cin <= k ->
-  (ρ, e, cin) ⇓cps (v, cout) ->
-  exists tenv' m',
-  (* then running stmt down to Sskip yields args[1] related to v at level k-j *)
-  (env, tenv, m, stmt) ⇓ (tenv', m') /\
-  match! tenv' ! args_id with Some (Vptr b o) in
-  match! Mem.load int_chunk m' b (index_offset o 1) with Some cv' in
-  rel_val (k - to_nat cin) v m' cv'.
-
-Definition Forall' := fold_right and True.
-Definition rel_val_aux (k : nat) :=
-  fix go (v : cps.val) (m : Memory.mem) (cv : Values.val) : Prop :=
-  match v, cv with
-  | Vint v, cv => cv = make_vint (rep_unboxed (Z.to_N v))
-  | Vconstr t vs, cv =>
-    match get_ctor_rep cenv t with
-    | Ret (enum t) => cv = make_vint (rep_unboxed t)
-    | Ret (boxed t a) =>
-      match! cv with Vptr b o in
-      Mem.load int_chunk m b (header_offset o) = Some (make_vint (rep_boxed t a)) /\
-      let arg_ok i v :=
-        (* TODO: do we only ever load memory in int_chunk chunks? if so, can define as helper function *)
-        match! Mem.load int_chunk m b (index_offset o (Z.of_N i)) with Some cv in
-        go v m cv
-      in Forall' (mapi arg_ok 0 vs)
-    | _ => False
-    end
-  | Vfun ρ fds f, Vptr b o =>
-    o = Ptrofs.zero /\
-    match! find_def f fds with Some (t, xs, e) in
-    match! fenv ! f with Some (arity, indices) in
-    Genv.find_symbol prog_genv f = Some b /\
-    match! Genv.find_funct prog_genv (Vptr b o) with Some (Internal fn) in
-    forall j vs m cvs ρ_xvs env tenv m_cvs_firstn args_b args_o,
-    j < k ->
-    match k with
-    | 0 => True
-    | S k =>
-      (* suppose that f is called with arguments vs and fn with arguments cvs, and that vs
-         and cvs are related at level j<k (written as k-(k-j) to convince Coq of well-foundedness). *)
-      let j := k-(k-j) in
-      Forall2 (fun v cv => rel_val j v m cv) vs cvs ->
-      (* if extend ρ with xs↦vs... *)
-      set_lists xs vs (def_funs fds fds ρ ρ) = Some ρ_xvs ->
-      (* and extend the C configuration with xs↦cvs... *)
-      tenv ! args_id = Some (Vptr args_b args_o) ->
-      let arg_ok cv i := Mem.load int_chunk m args_b (index_offset args_o (Z.of_N i)) = Some cv in
-      Forall2 arg_ok (skipn n_param cvs) (skipn n_param indices) ->
-      function_entry1 prog_genv fn (firstn n_param cvs) m env tenv m_cvs_firstn ->
-      (* then e is related to the body of fn at level j *)
-      rel_exp' j ρ e env tenv m_cvs_firstn (fn_body fn)
-    end
-  | _, _ => False
-  end.
-
-End CycleBreakers.
-
-(* L6 values are related to (C value, heap) pairs *)
-Fixpoint rel_val (k : nat) := fun v '(m, cv) => 
-  rel_val_aux (fun k v m cv => rel_val k v (m, cv)) k v m cv.
-Notation "v '~ᵥ{' k '}' cv" := (rel_val k v cv) (at level 80).
-
-(* L6 (environment, term) pairs are related to Clight (environment, heap, statement) triples *)
-Definition rel_exp (k : nat) := fun '(ρ, e) '(env, tenv, m, stmt) => 
-  rel_exp' (fun k v m cv => rel_val k v (m, cv)) k ρ e env tenv m stmt.
-Notation "e '~{' k '}' ce" := (rel_exp k e ce) (at level 80).
-
-(* L6 environments are related to (environment, heap) pairs wrt a set of identifiers S *)
-Definition rel_env k := fun S ρ '(env, tenv, m) =>
-  forall x, x \in S ->
-  match! ρ!x with Some v in
-  match tenv!x with
-  | Some v' => v ~ᵥ{k} (m, v')
-  | None =>
-    match! env!x : option (_ * type) with Some (b, _) in
-    v ~ᵥ{k} (m, Vptr b Ptrofs.zero)
-  end.
-Notation "ρ '~ₑ{' k ',' S '}' cρ" := (rel_env k S ρ cρ) (at level 80).
-Notation "ρ '~ₑ{' k '}' cρ" := (rel_env k (fun _ => True) ρ cρ) (at level 80).
-
-(** ** Antimonotonicity of the logical relation *)
-
-(* TODO: hoist and maybe find better way to express this theorem *)
-Lemma mapi_rel {A B} (R : B -> B -> Prop) op z (f g : _ -> A -> B) i (xs : list A) :
-  forall (Hfg_ok : forall i x, List.In x xs -> R (f i x) (g i x))
-    (HR_z_ok : R z z)
-    (HR_op_ok : forall x y x' y', R x y -> R x' y' -> R (op x x') (op y y')),
-  R (fold_right op z (mapi f i xs)) (fold_right op z (mapi g i xs)).
-Proof.
-  intros; revert i; induction xs as [|x xs IHxs]; cbn; [easy|]; intros i.
-  apply HR_op_ok; [apply Hfg_ok; now left|].
-  apply IHxs; intros i' x' Hin; apply Hfg_ok; now right.
-Qed.
-
-Fixpoint sizeof_val v :=
-  match v with
-  | Vconstr t vs => 1 + fold_right (fun v n => sizeof_val v + n) 0 vs
-  | Vfun ρ fds f => 1
-  | Vint _ => 0
-  end.
-Lemma rel_val_eqn k v m cv :
-  rel_val k v (m, cv) = rel_val_aux (fun k v m cv => rel_val k v (m, cv)) k v m cv.
-Proof. now destruct k. Qed.
-
-Lemma rel_val_antimon : forall j k v m cv,
-  j <= k ->
-  v ~ᵥ{k} (m, cv) ->
-  v ~ᵥ{j} (m, cv).
-Proof.
-  intros j k; revert j.
-  induction k as [k IHk] using lt_wf_ind.
-  intros j v; revert j.
-  remember (sizeof_val v) as sv eqn:Hsv; generalize dependent v.
-  induction sv as [sv IHsv] using lt_wf_ind.
-  intros v Hsv j m cv Hle.
-  rewrite !rel_val_eqn; destruct v as [t [|v vs] |ρ fds f|i].
-  - auto.
-  - cbn; destruct (get_ctor_rep _ _) as [| [tag|tag arity]] eqn:Hrep; auto.
-    destruct cv; auto; 
-    intros [Hload Hforall]; split; [easy|].
-    change (_ /\ Forall' (mapi ?f 1 _)) with (Forall' (mapi f 0 (v :: vs))) in *.
-    pose proof @mapi_rel val Prop (fun P Q => P -> Q) and True as mapi_rel.
-    specialize mapi_rel with (i := 0%N) (xs := v :: vs).
-    match goal with _ : Forall' (mapi ?f' _ _) |- _ => specialize mapi_rel with (f := f') end.
-    match goal with |- Forall' (mapi ?g' _ _) => specialize mapi_rel with (g := g') end.
-    apply mapi_rel; clear mapi_rel; [|tauto..].
-    intros i' x Hin.
-    destruct (Mem.load _ m b (index_offset i (Z.of_N i'))); [|tauto].
-    rewrite <- !rel_val_eqn; eapply IHsv; auto.
-    subst sv; destruct Hin as [[] |Hin]; [cbn; lia|clear - Hin].
-    induction vs as [|v' vs IHvs]; [easy|].
-    destruct Hin as [[] |Hin]; [cbn; lia|cbn in *; specialize (IHvs Hin); lia].
-  - simpl; destruct cv; auto.
-    destruct (find_def f fds) as [[[f' xs] e] |] eqn:Hfind; auto.
-    destruct (fenv ! f) as [[arity indices] |] eqn:Hindices; auto.
-    intros [Hi_zero Hrest]; split; [easy|]; revert Hrest.
-    intros [Hfind_symbol Hrest]; split; [easy|]; revert Hrest.
-    match goal with |- context [if ?e1 then ?e2 else ?e3] =>
-      change (if e1 then e2 else e3) with (Genv.find_funct prog_genv (Vptr b i));
-      destruct (Genv.find_funct prog_genv (Vptr b i)) as [[fn|] |] eqn:Hfind_funct; auto
-    end.
-    intros Hfuture_call; intros*; intros Hlt; destruct j; [easy|].
-    intros Hvs_firstn_ok Hcvs_firstn_ok Hvs_rest_ok Hcvs_rest_ok Hvs_related.
-    intros Hextend_ρ Hextend_args Hextend_locals Hentry.
-    replace (j - (j - j0)) with j0 in * by lia.
-    destruct k as [|k]; [lia|].
-    specialize Hfuture_call with (j := j0).
-    replace (k - (k - j0)) with j0 in Hfuture_call by lia.
-    eapply Hfuture_call; eauto; lia.
-  - auto.
-Qed.
-
-Lemma rel_exp_antimon j k ρ e env tenv m stmt :
-  j <= k ->
-  (ρ, e) ~{k} (env, tenv, m, stmt) ->
-  (ρ, e) ~{j} (env, tenv, m, stmt).
-Proof.
-  intros Hle Hk v cin cout Hcost Hbstep.
-  edestruct Hk as [tenv' [m' [Hsteps Hres]]]; eauto; [lia|].
-  exists tenv', m'; split; [eauto|].
-  destruct (tenv' ! args_id) as [[] |]; try contradiction.
-  destruct (Mem.load _ _ _ _); try contradiction.
-  eapply rel_val_antimon; [|eassumption]; lia.
-Qed.
-
-Lemma rel_env_antimon j k S ρ env tenv m :
-  j <= k ->
-  ρ ~ₑ{k, S} (env, tenv, m) ->
-  ρ ~ₑ{j, S} (env, tenv, m).
-Proof.
-  intros Hle Hk x Hx; specialize (Hk x Hx).
-  destruct (ρ ! x); [|easy].
-  destruct (tenv ! x); [eapply rel_val_antimon; eauto|].
-  destruct (env ! x) as [[] |]; [|easy].
-  eapply rel_val_antimon; eauto.
-Qed.
-
-Lemma rel_env_antimon_S k S1 S2 ρ env tenv m :
-  S1 \subset S2 ->
-  ρ ~ₑ{k, S2} (env, tenv, m) ->
-  ρ ~ₑ{k, S1} (env, tenv, m).
-Proof. intros Hle Hk x Hx; now apply Hk, Hle. Qed.
-
-(** ** Lemmas about the environment relation *)
-
-Lemma rel_env_gss k S x v cv ρ env tenv m :
-  x \in S ->
-  v ~ᵥ{k} (m, cv) ->
-  ρ ~ₑ{k, S \\ [set x]} (env, tenv, m) ->
-  M.set x v ρ ~ₑ{k, S} (env, M.set x cv tenv, m).
-Proof.
-  intros Hin Hv Hρ x' Hx'.
-  destruct (M.elt_eq x x') as [Heq|Hne]; [subst x'; now rewrite !M.gss|].
-  rewrite !M.gso by auto.
-  apply Hρ; constructor; [auto|now inversion 1].
-Qed.
-
-Lemma rel_env_gss_sing k x v cv ρ env tenv m :
-  v ~ᵥ{k} (m, cv) ->
-  M.set x v ρ ~ₑ{k, [set x]} (env, M.set x cv tenv, m).
-Proof.
-  intros Hv x' Hx'.
-  destruct (M.elt_eq x x') as [Heq|Hne]; [|now inv Hx'].
-  subst x'; now rewrite !M.gss.
-Qed.
-
-Lemma rel_env_gso k S x v cv ρ env tenv m :
-  ~ x \in S ->
-  ρ ~ₑ{k, S} (env, tenv, m) ->
-  M.set x v ρ ~ₑ{k, S} (env, M.set x cv tenv, m).
-Proof.
-  intros Hin Hρ x' Hx'.
-  destruct (M.elt_eq x x') as [Heq|Hne]; [easy|].
-  rewrite !M.gso by auto. now apply Hρ.
-Qed.
-
-Lemma rel_env_union k S1 S2 ρ env tenv m :
-  ρ ~ₑ{k, S1 :|: S2} (env, tenv, m) <->
-  ρ ~ₑ{k, S1} (env, tenv, m) /\ ρ ~ₑ{k, S2} (env, tenv, m).
-Proof.
-  split; [intros HS12|intros [HS1 HS2]].
-  - split; intros x Hx; now apply HS12.
-  - intros x Hx; inv Hx; [apply HS1|apply HS2]; easy.
-Qed.
-
-(** ** λ-ANF reductions preserve relatedness *)
-
-Ltac solve_rel_exp_reduction :=
-  unfold rel_exp, rel_exp'; intros Hweaker v cin cout Hk Hbstep;
-  inv Hbstep; match goal with | H : bstep _ _ _ _ _ _ |- _ => inv H end;
-  rewrite to_nat_add in *;
-  edestruct Hweaker as [tenv' [m' [Hstep Hresult]]]; [idtac..|eassumption|]; [idtac..|lia|]; eauto;
-  do 2 eexists; split; eauto;
-  destruct (tenv' ! args_id) as [[] |]; eauto;
-  destruct (Mem.load _ _ _ _); eauto;
-  eapply rel_val_antimon; [|eauto]; lia.
-
-Lemma rel_exp_constr k ρ x c ys e env tenv m stmt :
-  (forall vs,
-    get_list ys ρ = Some vs ->
-    (M.set x (Vconstr c vs) ρ, e) ~{k} (env, tenv, m, stmt)) ->
-  (ρ, Econstr x c ys e) ~{k} (env, tenv, m, stmt).
-Proof. solve_rel_exp_reduction. Qed.
-
-Lemma rel_exp_proj k ρ x c n y e env tenv m stmt :
-  (forall vs v,
-    ρ!y = Some (Vconstr c vs) ->
-    nthN vs n = Some v ->
-    (M.set x v ρ, e) ~{k} (env, tenv, m, stmt)) ->
-  (ρ, Eproj x c n y e) ~{k} (env, tenv, m, stmt).
-Proof. solve_rel_exp_reduction. Qed.
-
-Lemma rel_exp_case k ρ x ces env tenv m stmt :
-  (forall c vs n e,
-    ρ!x = Some (Vconstr c vs) ->
-    cps_util.caseConsistent cenv ces c ->
-    cps_util.find_tag_nth ces c e n ->
-    (ρ, e) ~{k} (env, tenv, m, stmt)) ->
-  (ρ, Ecase x ces) ~{k} (env, tenv, m, stmt).
-Proof. solve_rel_exp_reduction. Qed.
-
-Lemma rel_exp_app k ρ f t ys env tenv m stmt :
-  (forall ρ_f fds f' vs xs e ρ_f_xvs,
-    ρ!f = Some (Vfun ρ_f fds f') ->
-    get_list ys ρ = Some vs ->
-    find_def f' fds = Some (t, xs, e) ->
-    set_lists xs vs (def_funs fds fds ρ_f ρ_f) = Some ρ_f_xvs ->
-    (ρ_f_xvs, e) ~{k} (env, tenv, m, stmt)) ->
-  (ρ, Eapp f t ys) ~{k} (env, tenv, m, stmt).
-Proof. solve_rel_exp_reduction. Qed.
-
-Lemma rel_exp_prim k ρ x p ys e env tenv m stmt :
-  (ρ, Eprim x p ys e) ~{k} (env, tenv, m, stmt).
-Proof. intros v cin cout Hk Hrun; inv Hrun; inv H. Qed.
-
-(** ** Clight reductions preserve relatedness *)
-
-Lemma rel_exp_Cred env' tenv' m' stmt' k ρ e env tenv m stmt :
-  (env, tenv, m, stmt) --> (env', tenv', m', stmt') ->
-  (ρ, e) ~{k} (env', tenv', m', stmt') ->
-  (ρ, e) ~{k} (env, tenv, m, stmt).
-Proof.
-  unfold rel_exp; intros Hsimple_step Hrel v cin cout Hk Hbstep.
-  edestruct Hrel as [tenv'' [m'' [Hstep2_after Hres]]]; eauto.
-Qed.
-
-(* TODO: basically, want one rule for each C code fragment corresponding to an L6 reduction step *)
-
-(** * Relating λ-ANF calls to Clight calls *)
-
-(*
-
-Lemma rel_exp_letapp_compat k ρ x f t ys e env tenv m stmt :
-  (forall ρ_f fds f' vs xs e ρ_f_xvs v,
-    ρ!f = Some (Vfun ρ_f fds f') ->
-    get_list ys ρ = Some vs ->
-    find_def f' fds = Some (t, xs, e_f) ->
-    set_lists xs vs (def_funs fds fds ρ_f ρ_f) = Some ρ_f_xvs ->
-    (ρ_f_xvs, e_f, cin) ⇓f (v, cout) ->
-    (M.set x v ρ, e_f) ~{k} (env, tenv, m, stmt)) ->
-  (ρ, Eletapp x f t ys e) ~{k} (env, tenv, m, stmt).
-Proof. solve_rel_exp_reduction. Qed.
-
-*)
-
-(** * Main theorem *)
+(** * Basic facts about the code generator *)
 
 Lemma bind_ret {A B} x (f : A -> error B) : (x <- Ret x ;; f x) = f x.
 Proof. reflexivity. Qed.
@@ -1198,9 +828,6 @@ Arguments Monad.bind : simpl never.
 Arguments add_local_fvs : simpl never.
 Arguments exp_fv : simpl never.
 Arguments PS.cardinal : simpl never.
-Arguments rel_val : simpl never.
-Arguments rel_exp : simpl never.
-Arguments rel_env : simpl never.
 
 Ltac bind_step_in H x Hx :=
   match type of H with
@@ -1223,19 +850,19 @@ Proof.
   - rewrite FromSet_add.
     rewrite Intersection_Same_set; [apply Union_commut|].
     apply Singleton_Included.
-    eapply FromSet_complete; eauto with Ensembles_DB.
+    eapply FromSet_complete; sets.
   - assert (~ PS.In x locals) by (intros Hin'; now rewrite <- PS.mem_spec in Hin').
     assert (~ x \in FromSet locals) by (intros Hin'; now eapply FromSet_sound in Hin').
-    rewrite Intersection_Disjoint; eauto with Ensembles_DB.
+    rewrite Intersection_Disjoint; sets.
 Qed.
 
 Lemma add_local_fvs_ok locals fvs xs :
   FromSet (add_local_fvs locals fvs xs) <--> FromSet fvs :|: (FromList xs :&: FromSet locals).
 Proof.
   revert fvs; induction xs as [|x xs IHxs]; intros fvs.
-  - cbn; rewrite FromList_nil, Intersection_Empty_set_abs_l; eauto with Ensembles_DB.
+  - cbn; rewrite FromList_nil, Intersection_Empty_set_abs_l; sets.
   - unfold add_local_fvs in *; cbn; rewrite IHxs, add_local_fv_ok, FromList_cons.
-    rewrite Intersection_Union_distr; eauto with Ensembles_DB.
+    rewrite Intersection_Union_distr; sets.
 Qed.
 
 Lemma FromSet_remove x s : FromSet (PS.remove x s) <--> FromSet s \\ [set x].
@@ -1265,13 +892,13 @@ Proof.
     specialize (IHe locals nenv e); rewrite He in IHe;
     rewrite add_local_fvs_ok, FromSet_remove; normalize_occurs_free;
     rewrite Intersection_Union_distr, Union_commut;
-    apply Same_set_Union_compat; eauto with Ensembles_DB;
-    rewrite IHe, Intersection_extract_Setminus; eauto with Ensembles_DB.
+    apply Same_set_Union_compat; sets;
+    rewrite IHe, Intersection_extract_Setminus; sets.
   - cbn. bind_step cases Hcases; destruct cases as [[[??] fvs_cs] ?].
     rewrite add_local_fv_ok.
     revert dependent n; revert l0 l1 fvs_cs;
     induction l as [| [c e] ces IHces]; intros l0 l1 fvs_cs n Hcases; cbn in *.
-    + inv Hcases; rewrite FromSet_empty; normalize_occurs_free; eauto with Ensembles_DB.
+    + inv Hcases; rewrite FromSet_empty; normalize_occurs_free; sets.
     + bind_step_in Hcases e' He'; destruct e' as [[? fvs_e] ?].
       bind_step_in Hcases ces' Hces'; destruct ces' as [[[??]fvs_ces]?].
       specialize (IHces _ _ _ _ eq_refl).
@@ -1279,32 +906,32 @@ Proof.
       assert (fvs_cs = PS.union fvs_e fvs_ces) by (now destruct rep); subst.
       specialize (IHe locals nenv e); rewrite He' in IHe.
       normalize_occurs_free; rewrite FromSet_union, <- Union_assoc, IHces, IHe, !Intersection_Union_distr.
-      split; repeat apply Union_Included; eauto with Ensembles_DB.
+      split; repeat apply Union_Included; sets.
       eapply Included_trans; [|apply Included_Union_r].
-      apply Included_Intersection_compat; eauto with Ensembles_DB.
+      apply Included_Intersection_compat; sets.
   - cbn. bind_step e' He; destruct e' as [[? fvs_e]?].
     specialize (IHe locals nenv e); rewrite He in IHe.
     normalize_occurs_free; rewrite add_local_fv_ok, FromSet_remove, IHe.
     rewrite !Intersection_Union_distr, Union_commut.
-    apply Same_set_Union_compat; eauto with Ensembles_DB.
+    apply Same_set_Union_compat; sets.
     now rewrite Intersection_extract_Setminus.
   - cbn. bind_step e' He; destruct e' as [[? fvs_e]?].
     bind_step call Hcall; normalize_occurs_free.
     specialize (IHe locals nenv e); rewrite He in IHe.
     rewrite add_local_fvs_ok, FromSet_remove, IHe, FromList_cons, !Intersection_Union_distr, Union_commut.
-    apply Same_set_Union_compat; eauto with Ensembles_DB.
+    apply Same_set_Union_compat; sets.
     now rewrite Intersection_extract_Setminus.
   - exact I.
   - cbn. bind_step call Hcall. normalize_occurs_free.
     rewrite add_local_fvs_ok, FromList_cons, !Intersection_Union_distr, Union_commut, FromSet_empty.
-    split; repeat apply Union_Included; eauto with Ensembles_DB.
+    split; repeat apply Union_Included; sets.
   - cbn. bind_step e' He; destruct e' as [[? fvs_e]?].
     specialize (IHe locals nenv e); rewrite He in IHe.
     normalize_occurs_free; rewrite add_local_fvs_ok, FromSet_remove, IHe.
     rewrite !Intersection_Union_distr, Union_commut.
-    apply Same_set_Union_compat; eauto with Ensembles_DB.
+    apply Same_set_Union_compat; sets.
     now rewrite Intersection_extract_Setminus.
-  - cbn. normalize_occurs_free; rewrite add_local_fv_ok, FromSet_empty; eauto with Ensembles_DB.
+  - cbn. normalize_occurs_free; rewrite add_local_fv_ok, FromSet_empty; sets.
 Qed.
 
 Lemma max_ge_or m n p :
@@ -1361,15 +988,863 @@ Proof.
   - cbn. intros C x g gt ys e' Hsubterm; destruct C; inv Hsubterm.
 Qed.
 
+(** * Tools for reasoning about Clight *)
+
+(** The C program produced by the code generator *)
+Variable (prog : program).
+
+(** Its global environment *)
+Let prog_genv : genv := globalenv prog.
+
+(** ** "Reductions" in machine state *)
+
+(** Bigstep evaluation of statements: unlike exec_stmt,
+    - Force the trace to be empty
+    - Force outcome to be Out_normal (i.e., statement can't exit early
+      via return/break/continue) *)
+Definition texec := fun '(env, tenv, m, stmt) '(tenv', m') =>
+  exec_stmt prog_genv env tenv m stmt Events.E0 tenv' m' Out_normal.
+Infix "⇓" := texec (at level 80, no associativity).
+
+(** Bigstep evaluation of l- and r-values *)
+Definition eval_expr_operator := fun '(env, tenv, m, e) v =>
+  eval_expr prog_genv env tenv m e v.
+Definition eval_lvalue_operator := fun '(env, tenv, m, e) '(b, o) =>
+  eval_lvalue prog_genv env tenv m e b o.
+Infix "⇓ᵣ" := eval_expr_operator (at level 80).
+Infix "⇓ₗ" := eval_lvalue_operator (at level 80).
+
+(** (env1, tenv1, m1, stmt1) "reduces to" (env2, tenv2, m2, stmt2) if every terminating
+    execution starting from (env2, tenv2, m2, stmt2) can be used to construct an execution
+    starting from (env1, tenv1, m1, stmt1) *)
+Definition Clight_state_red := fun '(env1, tenv1, m1, stmt1) '(env2, tenv2, m2, stmt2) =>
+  forall tenv' m',
+  (env2, tenv2, m2, stmt2) ⇓ (tenv', m') ->
+  (env1, tenv1, m1, stmt1) ⇓ (tenv', m').
+Infix "-->" := Clight_state_red (at level 80).
+
+Lemma Cred_trans s1 s2 s3 :
+  s1 --> s2 -> s2 --> s3 -> s1 --> s3.
+Proof. destruct s1 as [[[??]?]?], s2 as [[[??]?]?], s3 as [[[??]?]?]; cbn; eauto. Qed.
+
+Lemma Cred_seq_assoc s1 s2 s3 env tenv m :
+  (env, tenv, m, ((s1; s2); s3)) --> (env, tenv, m, (s1; (s2; s3))).
+Proof.
+  intros tenv' m' Hs123; inv Hs123; [|contradiction].
+  inv H9; [|contradiction].
+  unfold "⇓"; rewrite <- H4, <- Events.Eapp_assoc; repeat (eapply exec_Sseq_1; eauto).
+Qed.
+
+Lemma Cred_seq_congl env tenv m s tenv' m' s' cont :
+  (env, tenv, m, s) --> (env, tenv', m', s') ->
+  (env, tenv, m, (s; cont)) --> (env, tenv', m', (s'; cont)).
+Proof.
+  intros Hs tenv'' m'' Hseq; unfold "-->", "⇓" in *; inv Hseq; [|easy].
+  let solve_assertion :=
+    unfold Events.E0, Events.Eapp in *;
+    destruct t1; cbn in *; congruence
+  in
+  assert (t1 = Events.E0) by solve_assertion;
+  assert (t2 = Events.E0) by solve_assertion;
+  subst.
+  eapply exec_Sseq_1; eauto.
+Qed.
+
+Lemma Cred_skip env tenv m s :
+  (env, tenv, m, (Sskip; s)) --> (env, tenv, m, s).
+Proof.
+  intros tenv' m' Hexec.
+  unfold "⇓"; change Events.E0 with (Events.Eapp Events.E0 Events.E0).
+  eapply exec_Sseq_1; [constructor|eauto].
+Qed.
+
+Lemma Cred_set env tenv m x a v :
+  (env, tenv, m, a) ⇓ᵣ v ->
+  (env, tenv, m, x ::= a) --> (env, M.set x v tenv, m, Sskip).
+Proof. intros; intros ?? Hexec; inv Hexec; econstructor; eauto. Qed.
+
+Lemma Cred_assign env tenv m a1 a2 v_pre v b o m' :
+  (env, tenv, m, a1) ⇓ₗ (b, o) ->
+  (env, tenv, m, a2) ⇓ᵣ v_pre ->
+  sem_cast v_pre (typeof a2) (typeof a1) m = Some v ->
+  assign_loc prog_genv (typeof a1) m b o v m' ->
+  (env, tenv, m, a1 :::= a2) --> (env, tenv, m', Sskip).
+Proof. intros; intros ?? Hexec; inv Hexec; econstructor; eauto. Qed.
+
+Lemma Cred_if env tenv m a v b s1 s2 :
+  (env, tenv, m, a) ⇓ᵣ v ->
+  bool_val v (typeof a) m = Some b ->
+  (env, tenv, m, Sifthenelse a s1 s2) -->
+  (env, tenv, m, if b then s1 else s2).
+Proof. intros; intros ???; econstructor; eauto. Qed.
+
+(** ** Memory & memory predicates *)
+
+(** The code generator only emits code that loads/stores in single-word chunks *)
+Definition word_chunk := if Archi.ptr64 then Mint64 else Mint32.
+Definition word_size := size_chunk word_chunk.
+Definition load m b o i := Mem.load word_chunk m b (o + word_size*i).
+Definition store m b o i v := Mem.store word_chunk m b (o + word_size*i) v.
+
+(** If 64-bit, Coq values will be represented using only Vlong, Vptr, and Vundef.
+    If 32-bit, Coq values will be represented using only Vint, Vptr, and Vundef. *)
+Definition val_wf v :=
+  if Archi.ptr64 then match v with Vundef | Vlong _ | Vptr _ _ => True | _ => False end
+  else match v with Vundef | Values.Vint _ | Vptr _ _ => True | _ => False end.
+
+Lemma val_wf_load_result v :
+  val_wf v -> Val.load_result word_chunk v = v.
+Proof.
+  unfold val_wf, Val.load_result, word_chunk;
+  now destruct v, Archi.ptr64.
+Qed.
+
+(** Memory satisfies a separating conjunction of formulas of the form
+      (b, o, i) ↦ [v1; ..; vn]
+    each representing a chunk of memory containing n word-sized values v1 .. vn
+    starting at location (block, offset + word_size*i) *)
+Definition chunk := (block * Z * Z * list Values.val)%type.
+Definition mpred := list chunk.
+
+Definition mapsto : _ -> _ -> chunk := fun '(b, o, i) vs => (b, o, i, vs).
+Infix "↦" := mapsto (at level 80).
+
+(** A chunk ((b, o, i) ↦ vs) is well-represented if
+    - Each v in vs is well-represented
+    - The lowest and highest offsets are both representable as word-sized integers *)
+Definition chunk_lower : chunk -> Z := fun '(b, o, i, vs) => (o + word_size*i)%Z.
+Definition chunk_upper : chunk -> Z := fun '((b, o, i, vs) as c) => 
+  (chunk_lower c + word_size * Z.of_nat (length vs))%Z.
+Definition chunk_denote : chunk -> mem -> Prop :=
+  fun '((b, o, init, vs) as c) m =>
+  (forall i v, get_ith vs i = Some v -> load m b o (i + init) = Some v) /\
+  All (map val_wf vs) /\
+  (chunk_lower c >= 0)%Z /\
+  (chunk_upper c < O.modulus)%Z.
+Infix "∈" := chunk_denote (at level 80).
+
+(** The locations spanned by a chunk *)
+Definition chunk_locs : chunk -> Ensemble (block * Z) :=
+  fun '((b, o, i, vs) as c) '(b', o') =>
+  (b = b' /\ chunk_lower c <= o' < chunk_upper c)%Z.
+
+Definition chunk_disjoint c1 c2 :=
+  Disjoint _ (chunk_locs c1) (chunk_locs c2).
+
+Fixpoint mutually_disjoint p :=
+  match p with
+  | [] => True
+  | c :: p => All (map (chunk_disjoint c) p) /\ mutually_disjoint p
+  end.
+
+Definition mem_locs m : Ensemble (block * Z) :=
+  fun '(b, o) => exists v, Mem.load Mint8unsigned m b o = Some v.
+
+(** A store m satisfies a separating conjunction c1 * .. * cn if
+    - Each chunk is well-represented
+    - The chunks are mutually disjoint
+    - The chunks are exhaustive: every location in m corresponds to some c_i *)
+Definition mpred_denote (m : mem) (p : mpred) : Prop :=
+  All (map (fun c => c ∈ m) p) /\
+  mutually_disjoint p /\
+  mem_locs m \subset Bigcup (map chunk_locs p).
+Infix "⊨" := mpred_denote (at level 80).
+
+Lemma concretize_word_size : (word_size = 4 \/ word_size = 8)%Z.
+Proof. unfold word_size, word_chunk; destruct Archi.ptr64; cbn; lia. Qed.
+
+Ltac superlia :=
+  repeat match goal with
+  | |- context [Z.of_nat ?e] =>
+    lazymatch goal with
+    | H : (0 <= Z.of_nat e)%Z |- _ => fail
+    | _ => pose proof (Zle_0_nat e)
+    end
+  | H : context [Z.of_nat ?e] |- _ =>
+    lazymatch goal with
+    | H : (0 <= Z.of_nat e)%Z |- _ => fail
+    | _ => pose proof (Zle_0_nat e)
+    end
+  | H : get_ith ?xs ?i = Some _ |- _ =>
+    lazymatch goal with
+    | H : (0 <= i < Z.of_nat (length xs))%Z |- _ => fail
+    | _ => pose proof (get_ith_range _ _ _ H)
+    end
+  | |- context [length (set_ith ?xs ?i ?y)] =>
+    lazymatch goal with
+    | H : length (set_ith xs i y) = length xs |- _ => fail
+    | _ => pose proof (set_ith_len y xs i)
+    end
+  | H : context [length (set_ith ?xs ?i ?y)] |- _ =>
+    lazymatch goal with
+    | H : length (set_ith xs i y) = length xs |- _ => fail
+    | _ => pose proof (set_ith_len y xs i)
+    end
+  end;
+  change (size_chunk word_chunk) with word_size in *;
+  rewrite ?Z.mul_add_distr_l, ?Z.mul_add_distr_r in *;
+  (pose proof concretize_word_size);
+  lia.
+
+Lemma chunk_cons b o init v vs m :
+  ((b, o, init) ↦ v :: vs) ∈ m ->
+  ((b, o, init+1)%Z ↦ vs) ∈ m.
+Proof.
+  intros [Hget [Hwf Hbounds]].
+  split; [|split; cbn in *; [easy|superlia]].
+  intros i v' Hget'. replace (i + (init + 1))%Z with ((i + 1) + init)%Z by lia.
+  apply Hget; cbn; destruct (Coqlib.zeq (i + 1)%Z 0).
+  - apply Coqlib.list_nth_z_range in Hget'; lia.
+  - rewrite <- Hget'; f_equal; lia.
+Qed.
+
+Lemma chunk_load m b o v : forall vs init i,
+  ((b, o, init) ↦ vs) ∈ m ->
+  get_ith vs (i - init) = Some v ->
+  load m b o i = Some v.
+Proof.
+  induction vs as [|v' vs IHvs]; [inversion 2|].
+  intros* Hchunk Hnth; cbn in Hnth.
+  destruct (Coqlib.zeq (i - init) 0) as [Heq|Hne].
+  - inv Hnth; assert (i = init) by lia; subst init.
+    now apply (proj1 Hchunk 0%Z).
+  - apply chunk_cons in Hchunk.
+    eapply IHvs; eauto.
+    rewrite <- Hnth; f_equal; lia.
+Qed.
+
+Arguments Z.of_nat : simpl never.
+Lemma chunk_store_same m m' b o v : forall vs init i,
+  val_wf v ->
+  (0 <= i < Z.of_nat (length vs))%Z ->
+  store m b o (i + init) v = Some m' ->
+  ((b, o, init) ↦ vs) ∈ m ->
+  ((b, o, init) ↦ set_ith vs i v) ∈ m'.
+Proof.
+  induction vs as [|v' vs IHvs]; [cbn; lia|intros* Hwf Hbound Hstore Hchunk].
+  rewrite set_ith_cons; destruct (Z.eq_dec i 0) as [|Hne]; [subst|].
+  - split; [intros i v'' Hget|split; cbn in *; [tauto|superlia]].
+    cbn in Hget; destruct (Coqlib.zeq i 0) as [|Hne]; [subst|].
+    + assert (val_wf v'') by now inv Hget.
+      inv Hget; rewrite <- (val_wf_load_result v'') by auto.
+      eapply Mem.load_store_same; eauto.
+    + apply chunk_cons in Hchunk.
+      apply Hchunk in Hget; rewrite <- Hget.
+      replace (Z.pred i + (init + 1))%Z with (i + init)%Z by lia.
+      eapply Mem.load_store_other; eauto; superlia.
+  - pose proof set_ith_len v vs (Z.pred i).
+    pose proof Hchunk as Hchunk_next; apply chunk_cons in Hchunk_next.
+    specialize (IHvs (init + 1)%Z (Z.pred i) Hwf).
+    replace (Z.pred i + (init + 1))%Z with (i + init)%Z in * by lia.
+    split; [intros j v'' Hget|split; [|cbn in *; superlia]].
+    + cbn in Hget; destruct (Coqlib.zeq j 0) as [|Hne']; [subst|].
+      * inv Hget. destruct Hchunk as [Hchunk _].
+        specialize (Hchunk 0%Z v'').
+        erewrite <- Hchunk by auto.
+        eapply Mem.load_store_other; eauto; superlia.
+      * destruct IHvs as [Hchunk' _]; auto; [cbn in *; superlia|].
+        specialize (Hchunk' _ _ Hget); rewrite <- Hchunk'; f_equal; lia.
+    + split; [cbn in *; tauto|].
+      destruct IHvs as [Hchunk' [Hwf' Hbounds']]; auto.
+      cbn in *; superlia.
+Qed.
+
+Lemma Disjoint_pair_simpl {A B} (S1 S2 : Ensemble (A * B)) :
+  Disjoint _ S1 S2 <-> forall x y, ~ (S1 (x, y) /\ S2 (x, y)).
+Proof.
+  split; [intros [Hdis] x y Hxy; now destruct (Hdis (x, y))|].
+  intros H; constructor; intros [x y] Hxy; apply (H x y); now inv Hxy.
+Qed.
+
+Lemma chunk_disjoint_simpl b1 o1 i1 vs1 b2 o2 i2 vs2 :
+  let c1 := (b1, o1, i1) ↦ vs1 in
+  let c2 := (b2, o2, i2) ↦ vs2 in
+  chunk_disjoint c1 c2 <->
+  b1 <> b2 \/
+  length vs1 = 0 \/
+  length vs2 = 0 \/
+  (chunk_upper c1 <= chunk_lower c2)%Z \/
+  (chunk_upper c2 <= chunk_lower c1)%Z.
+Proof.
+  remember ((b1, o1, i1) ↦ vs1) as c1; remember ((b2, o2, i2) ↦ vs2) as c2.
+  lazy zeta; rewrite Heqc1, Heqc2.
+  unfold "↦", chunk_disjoint, chunk_locs in *; rewrite Disjoint_pair_simpl.
+  split; [intros H|subst; cbn in *; superlia].
+  destruct (Pos.eq_dec b1 b2); [right|now left].
+  destruct (Nat.eq_dec (length vs1) 0); [now left|right].
+  destruct (Nat.eq_dec (length vs2) 0); [now left|right].
+  assert (chunk_lower c1 < chunk_upper c1)%Z by (subst; cbn in *; superlia).
+  assert (chunk_lower c2 < chunk_upper c2)%Z by (subst; cbn in *; superlia).
+  destruct (Z_le_dec (chunk_lower c1) (chunk_lower c2)).
+  + specialize (H b1 (chunk_lower c2)); subst; cbn in *; superlia.
+  + specialize (H b1 (chunk_lower c1)); subst; cbn in *; superlia.
+Qed.
+
+Lemma chunk_store_other m m' b o v vs init i : forall c,
+  (0 <= i < Z.of_nat (length vs))%Z ->
+  store m b o (i + init) v = Some m' ->
+  ((b, o, init) ↦ vs) ∈ m ->
+  c ∈ m ->
+  chunk_disjoint c ((b, o, init) ↦ vs) ->
+  c ∈ m'.
+Proof.
+  intros [[[b' o'] init'] vs'] Hbound Hstore Hdst [Hc_load [Hc_wf Hc_bounds]] Hdisjoint.
+  change (b', o', init', vs') with ((b', o', init') ↦ vs') in *.
+  split; [|split; auto].
+  intros i' v' Hget; erewrite <- Hc_load; eauto.
+  eapply Mem.load_store_other; eauto.
+  rewrite chunk_disjoint_simpl in Hdisjoint.
+  cbn in *; superlia.
+Qed.
+
+Arguments mapsto : simpl never.
+Lemma mpred_load m b o v vs init i : forall p q,
+  m ⊨ (p ++ ((b, o, init) ↦ vs) :: q)%list ->
+  get_ith vs (i - init) = Some v ->
+  load m b o i = Some v.
+Proof.
+  intros* Hsat Hget.
+  eapply chunk_load; eauto.
+  destruct Hsat as [Hsat _].
+  rewrite map_app, All_app in Hsat; cbn in Hsat; tauto.
+Qed.
+
+Lemma mutually_disjoint_app ps qs :
+  mutually_disjoint (ps ++ qs)%list <->
+  mutually_disjoint ps /\ mutually_disjoint qs /\
+  All (map (fun p => All (map (chunk_disjoint p) qs)) ps).
+Proof.
+  induction ps as [|p ps IHps]; cbn; [tauto|].
+  rewrite map_app, All_app, IHps; tauto.
+Qed.
+
+(* TODO hoist *)
+Lemma All_and {A} P Q (xs : list A) :
+  All (map (fun x => P x /\ Q x) xs) <-> All (map P xs) /\ All (map Q xs).
+Proof. induction xs; cbn; tauto. Qed.
+
+(* TODO hoist *)
+Lemma All_iff {A} P Q (xs : list A) :
+  (forall x, P x <-> Q x) ->
+  All (map P xs) <-> All (map Q xs).
+Proof. induction xs; cbn; firstorder. Qed.
+
+Lemma chunk_disjoint_com b1 o1 i1 vs1 b2 o2 i2 vs2 :
+  chunk_disjoint ((b1, o1, i1) ↦ vs1) ((b2, o2, i2) ↦ vs2) <->
+  chunk_disjoint ((b2, o2, i2) ↦ vs2) ((b1, o1, i1) ↦ vs1).
+Proof. rewrite !chunk_disjoint_simpl; lia. Qed.
+
+Lemma chunk_locs_set b o i vs j v :
+  chunk_locs ((b, o, i) ↦ set_ith vs j v) <--> chunk_locs ((b, o, i) ↦ vs).
+Proof. unfold "↦"; cbn; split; intros [b' o'] H; unfold In in *; superlia. Qed.
+
+Lemma chunk_disjoint_Same_set1 c c1 c2 :
+  chunk_locs c1 <--> chunk_locs c2 ->
+  chunk_disjoint c1 c <-> chunk_disjoint c2 c.
+Proof. unfold chunk_disjoint; intros ->; easy. Qed.
+
+Lemma chunk_disjoint_Same_set2 c c1 c2 :
+  chunk_locs c1 <--> chunk_locs c2 ->
+  chunk_disjoint c c1 <-> chunk_disjoint c c2.
+Proof. unfold chunk_disjoint; intros ->; easy. Qed.
+
+Lemma mpred_store m m' b o v vs init i : forall p q,
+  val_wf v ->
+  (0 <= i < Z.of_nat (length vs))%Z ->
+  store m b o (i + init) v = Some m' ->
+  m ⊨ (p ++ ((b, o, init) ↦ vs) :: q)%list ->
+  m' ⊨ (p ++ ((b, o, init) ↦ set_ith vs i v) :: q)%list.
+Proof.
+  intros* Hwf Hbound Hstore [Hchunks [Hsep Hcover]]; unfold "⊨".
+  rewrite !map_app, !All_app, !map_cons, !All_cons, !Bigcup_app, !Bigcup_cons in *.
+  rewrite mutually_disjoint_app in *; cbn in *.
+  rewrite All_and in Hsep.
+  assert (Hunchanged : forall p,
+           All (map (fun c => c ∈ m) p) ->
+           All (map (fun c => chunk_disjoint c ((b, o, init) ↦ vs)) p)
+           ->
+           All (map (fun c => c ∈ m') p)).
+  { intros r Hall Hdisjoint'; induction r as [|r Hr]; [easy|].
+    cbn in *; split; [|tauto]. eapply chunk_store_other; eauto; tauto. }
+  rewrite All_and; (repeat match goal with |- _ /\ _ => split end); try tauto.
+  - apply Hunchanged; tauto.
+  - eapply chunk_store_same; eauto; tauto.
+  - apply Hunchanged; [tauto|].
+    eapply All_iff; [intros [[[??]?]?]; apply chunk_disjoint_com|]; tauto.
+  - eapply All_iff; [intros c; apply chunk_disjoint_Same_set1, chunk_locs_set|]; tauto.
+  - eapply All_iff; [intros c; apply chunk_disjoint_Same_set2, chunk_locs_set|]; tauto.
+  - enough (Hsame : mem_locs m' <--> mem_locs m) by now rewrite Hsame, chunk_locs_set.
+    pose (P := 
+      fun (b' : block) j =>
+      let o := (o + word_size * (i + init))%Z in
+      ~ (b = b' /\ o <= j < o + word_size)%Z).
+    pose proof Hstore as Hsame.
+    apply (Mem.store_unchanged_on P) in Hsame; [|subst P; lazy zeta; superlia].
+    split; intros [b' o']; unfold mem_locs, In; intros [v' Hbo']; eauto with mem.
+Qed.
+
+(** The Clight machine state looks as follows at function entry:
+      temporary environment
+        tinfo_id ↦ (tinfo_b, tinfo_o)
+        frame_id ↦ (frame_b, frame_o)
+        alloc_id ↦ (nursery_b, alloc_o)
+        limit_id ↦ (nursery_b, limit_o)
+        args_id ↦ (args_b, args_o)
+        roots_id ↦ (roots_b, roots_o)
+      memory
+        (tinfo_b, tinfo_b) ↦ [_, _, _, (args_b, args_o), (fp_b, fp_o), nalloc]
+        (nursery_b, alloc_o) ↦ [_ × (limit_o - alloc_o)]
+        (roots_b, roots_o) ↦ [_ × size]
+        (frame_b, frame_o) ↦ [_, _, _]
+        (args_b, args_o) ↦ [_ × max_args]
+    where
+      nalloc ≥ max_allocs(L6 term to execute)
+      size ≥ |FV(e)| for all subterms (let y = f(xs) in e) of the L6 term to execute
+    (Assuming that parameters have all been stored in temporary variables and that
+     alloc/limit/etc have been fetched from tinfo)
+
+    During execution, the free space (nursery_b, [alloc_o, limit_o)) may shrink and
+    the temporary environment accumulates bindings for intermediate values.
+
+    Before calling a function f,
+    - tinfo is updated with the new alloc and limit
+    - values live across the call are pushed onto the shadow stack
+    - (skin n_param arguments) are stored in the args array at the indices specified by
+      f's calling convention
+    Now the state looks like (only relevant changes shown):
+      temp
+        ‥ bindings for intermediate values ‥
+      mem
+        (tinfo_b, tinfo_b) ↦ [(nursery_b, alloc_o), (nursery_b, limit_o), _, (args_b, args_o), (frame_b, frame_o), nalloc]
+        (roots_b, roots_o) ↦ [pushed Coq values ‥]
+        (frame_b, frame_o) ↦ [(roots_b, roots_o + |pushed Coq values|), (roots_b, roots_o), (fp_b, fp_o)]
+        (args_b, args_o) ↦ [‥ (skipn n_param ys) at indices specified by calling convention ‥]
+
+    After calling f(ys):
+      mem
+        (tinfo_b, tinfo_b) ↦ [(nursery_b, alloc_o), (nursery_b, limit_o), _, (args_b, args_o), (frame_b, frame_o), nalloc]
+        (roots_b, roots_o) ↦ [pushed Coq values' ‥]
+        (frame_b, frame_o) ↦ [(roots_b, roots_o + |pushed Coq values'|), (roots_b, roots_o), (fp_b, fp_o)]
+        (args_b, args_o) ↦ [‥ f(ys) at index 1 ‥]
+      where
+        pushed Coq values' still represents the Coq values pushed before the call, but may have moved by GC
+    
+    After garbage collection and popping everything back out:
+      mem
+        (tinfo_b, tinfo_b) ↦ [(nursery_b, alloc_o), (nursery_b, limit_o), _, (args_b, args_o), (fp_b, fp_o), nalloc]
+        (nursery_b, alloc_o) ↦ [_ × (limit_o - alloc_o)]
+        (roots_b, roots_o) ↦ [_ × size]
+        (frame_b, frame_o) ↦ [_, _, _]
+        (args_b, args_o) ↦ [_ × max_args]
+
+    At each step, each of the chunks listed under "mem" are mutually disjoint, and also disjoint from the CertiCoq heap.
+*)
+
+Notation "'match!' e1 'with' p 'in' e2" :=
+  (match e1 with p => e2 | _ => False end)
+  (at level 80, p pattern, e1 at next level, right associativity).
+
+(** Predicates on the temp environment *)
+Definition tpred := temp_env -> Prop.
+Definition tmapsto x v : tpred := fun tenv => tenv!x = Some v.
+
+(** *** Chunks of memory *)
+
+
+Definition chunk := (block * ptrofs * list Values.val)%type.
+
+Definition mpred := mem -> Prop.
+Definition mmapsto : _ -> _ -> mpred := fun '(b, o, i) vs =>
+  All (mapi (fun i v => load m b (index_offset o i) = Some v) i vs).
+
+Definition addrs := Ensemble (block * Z).
+Definition Addrs m : addrs :=
+  fun '(b, o) => match load m b o with Some _ => True | None => False end.
+
+Definition temp_mapsto := fun x v (tenv : temp_env) => tenv!x = Some v.
+Definition mem_mapsto := fun '(b, o, i) vs m => 
+  All (mapi (fun i v => load m b (index_offset o i) = Some v) i vs).
+Definition lift_and {A} p q (x : A) := p x /\ q x.
+
+Declare Scope pred_scope.
+Delimit Scope pred_scope with P.
+Infix "↦" := temp_mapsto (at level 80) : pred_scope.
+Infix "↦ₘ" := mem_mapsto (at level 80) : pred_scope.
+Infix "," := lift_and (at level 100) : pred_scope.
+
+Definition pred := temp_env -> mem -> Prop.
+Definition make_pred temp_pred mem_pred : pred :=
+  fun tenv m => temp_pred tenv /\ mem_pred m.
+Notation "'{' T ';' M '}'" := (make_pred T M).
+
+Definition 
+
+(** * Logical relation between λ-ANF and Clight *)
+
+Definition make_vint (z : Z) : Values.val :=
+  if Archi.ptr64
+  then Vlong (Int64.repr z)
+  else Values.Vint (Int.repr z).
+
+Fixpoint closed_val (v : cps.val) :=
+  match v with
+  | Vconstr c vs => fold_right (fun v P => closed_val v /\ P) True vs
+  | Vfun ρ fds f => M.bempty ρ = true
+  | Vint _ => True
+  end.
+
+Context {fuel : Type} {Hf : @fuel_resource fuel} {trace : Type} {Ht : @trace_resource trace}.
+
+Context (one_app_nonzero : forall f ft ys, to_nat (one (Eapp f ft ys)) > 0).
+
+(** Bigstep evaluation of L6 terms *)
+Definition bstep_res := fun '(ρ, e, cin) '(v, cout) =>
+  bstep_fuel cenv ρ e cin (Res v) cout.
+Infix "⇓cps" := bstep_res (at level 80).
+
+Section CycleBreakers.
+
+Context (rel_val : forall (k : nat) (v : cps.val) (m : Memory.mem) (cv : Values.val), Prop).
+
+Definition rel_exp' k (ρ : env) (e : cps.exp) env tenv m stmt : Prop :=
+  forall v (cin : fuel) (cout : trace),
+  (** if running e in environment ρ yields a value v in j <= k cost, *)
+  to_nat cin <= k ->
+  (ρ, e, cin) ⇓cps (v, cout) ->
+  (* m, tenv is a valid CertiCoq heap (alloc, limit, roots, ...)
+     roots array represents some values -> *)
+  exists tenv' m',
+  (** then running stmt down to Sskip yields args[1] related to v at level k-j *)
+  (env, tenv, m, stmt) ⇓ (tenv', m') /\
+  (* TODO: this should be tinfo->args[1], not args[1] *)
+  match! tenv' ! args_id with Some (Vptr b o) in
+  match! load m' b (index_offset o 1) with Some cv' in
+  rel_val (k - to_nat cin) v m' cv'.
+  (* m', tenv' is a valid CertiCoq heap and roots array represents same values *)
+
+Definition rel_val_aux (k : nat) :=
+  fix go (v : cps.val) (m : Memory.mem) (cv : Values.val) : Prop :=
+  match v, cv with
+  | Vint v, cv => cv = make_vint (rep_unboxed (Z.to_N v))
+  | Vconstr t vs, cv =>
+    match get_ctor_rep cenv t with
+    | Ret (enum t) => cv = make_vint (rep_unboxed t)
+    | Ret (boxed t a) =>
+      match! cv with Vptr b o in
+      load m b (index_offset o (-1)) = Some (make_vint (rep_boxed t a)) /\
+      let arg_ok i v :=
+        match! load m b (index_offset o i) with Some cv in
+        go v m cv
+      in All (mapi arg_ok 0 vs)
+    | _ => False
+    end
+  | Vfun ρ fds f, Vptr b o =>
+    o = O.zero /\
+    match! find_def f fds with Some (t, xs, e) in
+    match! fenv ! f with Some (arity, indices) in
+    Genv.find_symbol prog_genv f = Some b /\
+    match! Genv.find_funct prog_genv (Vptr b o) with Some (Internal fn) in
+    forall j vs m cvs ρ_xvs env tenv m_cvs_firstn args_b args_o,
+    j < k ->
+    match k with
+    | 0 => True
+    | S k =>
+      (** suppose that f is called with arguments vs and fn with arguments cvs, and that vs
+         and cvs are related at level j<k (written as k-(k-j) to convince Coq of well-foundedness). *)
+      let j := k-(k-j) in
+      Forall2 (fun v cv => rel_val j v m cv) vs cvs ->
+      (** if extend ρ with xs↦vs... *)
+      set_lists xs vs (def_funs fds fds ρ ρ) = Some ρ_xvs ->
+      (** and extend the C configuration with xs↦cvs... *)
+      tenv ! args_id = Some (Vptr args_b args_o) ->
+      (* TODO: this is wrong; should be indices specified by calling convention *)
+      let arg_ok cv i := load m args_b (index_offset args_o (Z.of_N i)) = Some cv in
+      Forall2 arg_ok (skipn n_param cvs) (skipn n_param indices) ->
+      function_entry1 prog_genv fn (firstn n_param cvs) m env tenv m_cvs_firstn ->
+      (** then e is related to the body of fn at level j *)
+      rel_exp' j ρ_xvs e env tenv m_cvs_firstn (fn_body fn)
+    end
+  | _, _ => False
+  end.
+
+End CycleBreakers.
+
+(** L6 values are related to (C value, heap) pairs *)
+Fixpoint rel_val (k : nat) := fun v '(m, cv) => 
+  rel_val_aux (fun k v m cv => rel_val k v (m, cv)) k v m cv.
+Notation "v '~ᵥ{' k '}' cv" := (rel_val k v cv) (at level 80).
+
+(** L6 (environment, term) pairs are related to Clight (environment, heap, statement) triples *)
+Definition rel_exp (k : nat) := fun '(ρ, e) '(env, tenv, m, stmt) => 
+  rel_exp' (fun k v m cv => rel_val k v (m, cv)) k ρ e env tenv m stmt.
+Notation "e '~{' k '}' ce" := (rel_exp k e ce) (at level 80).
+
+(** L6 environments are related to (temp environment, heap) pairs wrt a set of identifiers S.
+
+    Note: we require all identifiers in ρ to be in the temp environment only.
+    The local environment env is used by the bigstep semantics to hold values for function parameters.
+    TODO To move these values into tenv, the code generator loads each parameter into a temporary on
+    function entry.
+
+    The reason env shows up at all, in rel_exp, is to support linking with hand-written C code.
+    Someone may want to prove that their C code implements an L6 function; the extra env parameter
+    will let them do that without having to rewrite their C code to put all function parameters
+    into temporaries before using them. *)
+Definition rel_env k := fun S ρ '(tenv, m) =>
+  forall x, x \in S ->
+  match! ρ!x with Some v in
+  match! tenv!x with Some cv in
+  v ~ᵥ{k} (m, cv).
+Notation "ρ '~ₑ{' k ',' S '}' tenv" := (rel_env k S ρ tenv) (at level 80).
+Notation "ρ '~ₑ{' k '}' tenv" := (rel_env k (fun _ => True) ρ tenv) (at level 80).
+
+(** ** Antimonotonicity of the logical relation *)
+
+(* TODO: hoist and maybe find better way to express this theorem *)
+Lemma mapi_rel {A B} (R : B -> B -> Prop) op z (f g : _ -> A -> B) i (xs : list A) :
+  forall (Hfg_ok : forall i x, List.In x xs -> R (f i x) (g i x))
+    (HR_z_ok : R z z)
+    (HR_op_ok : forall x y x' y', R x y -> R x' y' -> R (op x x') (op y y')),
+  R (fold_right op z (mapi f i xs)) (fold_right op z (mapi g i xs)).
+Proof.
+  intros; revert i; induction xs as [|x xs IHxs]; cbn; [easy|]; intros i.
+  apply HR_op_ok; [apply Hfg_ok; now left|].
+  apply IHxs; intros i' x' Hin; apply Hfg_ok; now right.
+Qed.
+
+Fixpoint sizeof_val v :=
+  match v with
+  | Vconstr t vs => 1 + fold_right (fun v n => sizeof_val v + n) 0 vs
+  | Vfun ρ fds f => 1
+  | Vint _ => 0
+  end.
+Lemma rel_val_eqn k v m cv :
+  rel_val k v (m, cv) = rel_val_aux (fun k v m cv => rel_val k v (m, cv)) k v m cv.
+Proof. now destruct k. Qed.
+
+Lemma rel_val_antimon : forall j k v m cv,
+  j <= k ->
+  v ~ᵥ{k} (m, cv) ->
+  v ~ᵥ{j} (m, cv).
+Proof.
+  intros j k; revert j.
+  induction k as [k IHk] using lt_wf_ind.
+  intros j v; revert j.
+  remember (sizeof_val v) as sv eqn:Hsv; generalize dependent v.
+  induction sv as [sv IHsv] using lt_wf_ind.
+  intros v Hsv j m cv Hle.
+  rewrite !rel_val_eqn; destruct v as [t [|v vs] |ρ fds f|i].
+  - auto.
+  - cbn; destruct (get_ctor_rep _ _) as [| [tag|tag arity]] eqn:Hrep; auto.
+    destruct cv; auto; 
+    intros [Hload Hforall]; split; [easy|].
+    change (_ /\ All (mapi ?f 1 _)) with (All (mapi f 0 (v :: vs))) in *.
+    pose proof @mapi_rel val Prop (fun P Q => P -> Q) and True as mapi_rel.
+    specialize mapi_rel with (i := 0%Z) (xs := v :: vs).
+    match goal with _ : All (mapi ?f' _ _) |- _ => specialize mapi_rel with (f := f') end.
+    match goal with |- All (mapi ?g' _ _) => specialize mapi_rel with (g := g') end.
+    apply mapi_rel; clear mapi_rel; [|tauto..].
+    intros i' x Hin.
+    destruct (load m b (index_offset i i')); [|tauto].
+    rewrite <- !rel_val_eqn; eapply IHsv; auto.
+    subst sv; destruct Hin as [[] |Hin]; [cbn; lia|clear - Hin].
+    induction vs as [|v' vs IHvs]; [easy|].
+    destruct Hin as [[] |Hin]; [cbn; lia|cbn in *; specialize (IHvs Hin); lia].
+  - simpl; destruct cv; auto.
+    destruct (find_def f fds) as [[[f' xs] e] |] eqn:Hfind; auto.
+    destruct (fenv ! f) as [[arity indices] |] eqn:Hindices; auto.
+    intros [Hi_zero Hrest]; split; [easy|]; revert Hrest.
+    intros [Hfind_symbol Hrest]; split; [easy|]; revert Hrest.
+    match goal with |- context [if ?e1 then ?e2 else ?e3] =>
+      change (if e1 then e2 else e3) with (Genv.find_funct prog_genv (Vptr b i));
+      destruct (Genv.find_funct prog_genv (Vptr b i)) as [[fn|] |] eqn:Hfind_funct; auto
+    end.
+    intros Hfuture_call; intros*; intros Hlt; destruct j; [easy|].
+    intros Hvs_firstn_ok Hcvs_firstn_ok Hvs_rest_ok Hcvs_rest_ok Hvs_related.
+    intros Hextend_ρ Hextend_args Hextend_locals Hentry.
+    replace (j - (j - j0)) with j0 in * by lia.
+    destruct k as [|k]; [lia|].
+    specialize Hfuture_call with (j := j0).
+    replace (k - (k - j0)) with j0 in Hfuture_call by lia.
+    eapply Hfuture_call; eauto; lia.
+  - auto.
+Qed.
+
+Lemma rel_exp_antimon j k ρ e env tenv m stmt :
+  j <= k ->
+  (ρ, e) ~{k} (env, tenv, m, stmt) ->
+  (ρ, e) ~{j} (env, tenv, m, stmt).
+Proof.
+  intros Hle Hk v cin cout Hcost Hbstep.
+  edestruct Hk as [tenv' [m' [Hsteps Hres]]]; eauto; [lia|].
+  exists tenv', m'; split; [eauto|].
+  destruct (tenv' ! args_id) as [[] |]; try contradiction.
+  destruct (load _ _ _); try contradiction.
+  eapply rel_val_antimon; [|eassumption]; lia.
+Qed.
+
+Lemma rel_env_antimon j k S ρ tenv m :
+  j <= k ->
+  ρ ~ₑ{k, S} (tenv, m) ->
+  ρ ~ₑ{j, S} (tenv, m).
+Proof.
+  intros Hle Hk x Hx; specialize (Hk x Hx).
+  destruct (ρ ! x); [|easy].
+  destruct (tenv ! x); [eapply rel_val_antimon; eauto|easy].
+Qed.
+
+Lemma rel_env_antimon_S k S1 S2 ρ tenv m :
+  S1 \subset S2 ->
+  ρ ~ₑ{k, S2} (tenv, m) ->
+  ρ ~ₑ{k, S1} (tenv, m).
+Proof. intros Hle Hk x Hx; now apply Hk, Hle. Qed.
+
+(** ** Lemmas about the environment relation *)
+
+Lemma rel_env_gss k S x v cv ρ tenv m :
+  x \in S ->
+  v ~ᵥ{k} (m, cv) ->
+  ρ ~ₑ{k, S \\ [set x]} (tenv, m) ->
+  M.set x v ρ ~ₑ{k, S} (M.set x cv tenv, m).
+Proof.
+  intros Hin Hv Hρ x' Hx'.
+  destruct (M.elt_eq x x') as [Heq|Hne]; [subst x'; now rewrite !M.gss|].
+  rewrite !M.gso by auto.
+  apply Hρ; constructor; [auto|now inversion 1].
+Qed.
+
+Lemma rel_env_gss_sing k x v cv ρ tenv m :
+  v ~ᵥ{k} (m, cv) ->
+  M.set x v ρ ~ₑ{k, [set x]} (M.set x cv tenv, m).
+Proof.
+  intros Hv x' Hx'.
+  destruct (M.elt_eq x x') as [Heq|Hne]; [|now inv Hx'].
+  subst x'; now rewrite !M.gss.
+Qed.
+
+Lemma rel_env_gso k S x v cv ρ tenv m :
+  ~ x \in S ->
+  ρ ~ₑ{k, S} (tenv, m) ->
+  M.set x v ρ ~ₑ{k, S} (M.set x cv tenv, m).
+Proof.
+  intros Hin Hρ x' Hx'.
+  destruct (M.elt_eq x x') as [Heq|Hne]; [easy|].
+  rewrite !M.gso by auto. now apply Hρ.
+Qed.
+
+Lemma rel_env_union k S1 S2 ρ tenv m :
+  ρ ~ₑ{k, S1 :|: S2} (tenv, m) <->
+  ρ ~ₑ{k, S1} (tenv, m) /\ ρ ~ₑ{k, S2} (tenv, m).
+Proof.
+  split; [intros HS12|intros [HS1 HS2]].
+  - split; intros x Hx; now apply HS12.
+  - intros x Hx; inv Hx; [apply HS1|apply HS2]; easy.
+Qed.
+
+(** ** λ-ANF reductions preserve relatedness *)
+
+Ltac solve_rel_exp_reduction :=
+  unfold rel_exp, rel_exp'; intros Hweaker v cin cout Hk Hbstep;
+  inv Hbstep; match goal with | H : bstep _ _ _ _ _ _ |- _ => inv H end;
+  rewrite to_nat_add in *;
+  edestruct Hweaker as [tenv' [m' [Hstep Hresult]]]; [idtac..|eassumption|]; [idtac..|lia|]; eauto;
+  do 2 eexists; split; eauto;
+  destruct (tenv' ! args_id) as [[] |]; eauto;
+  destruct (load _ _ _); eauto;
+  eapply rel_val_antimon; [|eauto]; lia.
+
+Lemma rel_exp_constr k ρ x c ys e env tenv m stmt :
+  (forall vs,
+    get_list ys ρ = Some vs ->
+    (M.set x (Vconstr c vs) ρ, e) ~{k} (env, tenv, m, stmt)) ->
+  (ρ, Econstr x c ys e) ~{k} (env, tenv, m, stmt).
+Proof. solve_rel_exp_reduction. Qed.
+
+Lemma rel_exp_proj k ρ x c n y e env tenv m stmt :
+  (forall vs v,
+    ρ!y = Some (Vconstr c vs) ->
+    nthN vs n = Some v ->
+    (M.set x v ρ, e) ~{k} (env, tenv, m, stmt)) ->
+  (ρ, Eproj x c n y e) ~{k} (env, tenv, m, stmt).
+Proof. solve_rel_exp_reduction. Qed.
+
+Lemma rel_exp_case k ρ x ces env tenv m stmt :
+  (forall c vs n e,
+    ρ!x = Some (Vconstr c vs) ->
+    cps_util.caseConsistent cenv ces c ->
+    cps_util.find_tag_nth ces c e n ->
+    (ρ, e) ~{k} (env, tenv, m, stmt)) ->
+  (ρ, Ecase x ces) ~{k} (env, tenv, m, stmt).
+Proof. solve_rel_exp_reduction. Qed.
+
+Lemma rel_exp_app k ρ f t ys env tenv m stmt :
+  (forall k_f ρ_f fds f' vs xs e ρ_f_xvs,
+    k = S k_f ->
+    ρ!f = Some (Vfun ρ_f fds f') ->
+    get_list ys ρ = Some vs ->
+    find_def f' fds = Some (t, xs, e) ->
+    set_lists xs vs (def_funs fds fds ρ_f ρ_f) = Some ρ_f_xvs ->
+    (ρ_f_xvs, e) ~{k_f} (env, tenv, m, stmt)) ->
+  (ρ, Eapp f t ys) ~{k} (env, tenv, m, stmt).
+Proof.
+  intros Hsimpler v cin cout Hk Heval; inv Heval; inv H.
+  rewrite to_nat_add in *; specialize (one_app_nonzero f t ys).
+  assert (to_nat cin0 <= k - 1) by lia.
+  assert (Hk_f : exists k_f, k = S k_f) by (destruct k as [|k]; [|exists k]; lia).
+  destruct Hk_f as [k_f Heq].
+  edestruct Hsimpler as [tenv' [m' [Heval' Hresult]]]; eauto; try lia.
+  exists tenv', m'; split; [auto|].
+  destruct (tenv' ! args_id) as [[] |]; try contradiction.
+  destruct (load _ _ _); [|easy].
+  eapply rel_val_antimon; [|eauto]; lia.
+Qed.
+
+Lemma rel_exp_prim k ρ x p ys e env tenv m stmt :
+  (ρ, Eprim x p ys e) ~{k} (env, tenv, m, stmt).
+Proof. intros v cin cout Hk Hrun; inv Hrun; inv H. Qed.
+
+(** ** Clight reductions preserve relatedness *)
+
+Lemma rel_exp_Cred env' tenv' m' stmt' k ρ e env tenv m stmt :
+  (env, tenv, m, stmt) --> (env', tenv', m', stmt') ->
+  (ρ, e) ~{k} (env', tenv', m', stmt') ->
+  (ρ, e) ~{k} (env, tenv, m, stmt).
+Proof.
+  unfold rel_exp; intros Hsimple_step Hrel v cin cout Hk Hbstep.
+  edestruct Hrel as [tenv'' [m'' [Hstep2_after Hres]]]; eauto.
+Qed.
+
+(** Fully right-associate all [;]s *)
+Ltac norm_seq := repeat progress (eapply rel_exp_Cred; [apply Cred_seq_assoc|]).
+
+(** Step from _ ~{k} (env, tenv, m, (s; cont))
+    to _ ~{k} (env, tenv', m', cont)
+    using [lemma : (env, tenv, m, s) --> (env, tenv', m', Sskip)] *)
+Ltac Cstep lemma :=
+  eapply rel_exp_Cred; [eapply Cred_trans; [eapply Cred_seq_congl, lemma|apply Cred_skip] |].
+
+(** Ditto, but without the cont *)
+Ltac Cstep' lemma := eapply rel_exp_Cred; [eapply lemma|].
+
+(** * Main theorem *)
+
+Arguments rel_val : simpl never.
+Arguments rel_exp : simpl never.
+Arguments rel_env : simpl never.
+
+Ltac normalize_occurs_free_in H :=
+  eapply rel_env_antimon_S in H; [|normalize_occurs_free; apply Included_refl].
+
 Lemma translate_body_stm locals nenv k : forall e,
   match translate_body cenv fenv locals nenv e with
   | Ret (stmt, _, _) => forall ρ env tenv m,
-    ρ ~ₑ{k, occurs_free e} (env, tenv, m) ->
+    ρ ~ₑ{k, occurs_free e} (tenv, m) ->
     (* TODO: extra assumptions *)
     (ρ, e) ~{k} (env, tenv, m, stmt)
   | _ => True
   end.
 Proof.
+  (* TODO: induction on step index by not be necessary *)
   induction k as [k IHk] using lt_wf_ind; fix IHe 1; destruct e.
   - (* let x = Con c ys in e *)
     rename v into x, l into ys; cbn.
@@ -1378,11 +1853,10 @@ Proof.
       bind_step e' He; destruct e' as [[stm_e fvs_e] n_e].
       intros ρ env tenv m Hρ.
       apply rel_exp_constr; intros vs Hget.
-      eapply rel_exp_Cred; [apply Cred_set; now constructor|].
+      Cstep Cred_set; [constructor|].
       specialize (IHe e); rewrite He in IHe; apply IHe. Guarded.
-      eapply rel_env_antimon_S.
-      { apply (Included_Union_Setminus _ [set x]); eauto with Decidable_DB. }
-      eapply rel_env_antimon_S in Hρ; [|normalize_occurs_free; apply Included_refl].
+      eapply rel_env_antimon_S; [apply (Included_Union_Setminus _ [set x]); sets|].
+      normalize_occurs_free_in Hρ.
       rewrite rel_env_union in Hρ; destruct Hρ as [_ Hρ].
       rewrite rel_env_union; split; [apply rel_env_gso; [intros Hin; now inv Hin|auto] |].
       apply rel_env_gss_sing; rewrite rel_val_eqn; cbn; now rewrite Hrep.
@@ -1390,12 +1864,11 @@ Proof.
       bind_step e' He; destruct e' as [[stm_e fvs_e] n_e].
       intros ρ env tenv m Hρ.
       apply rel_exp_constr; intros vs Hget.
-      repeat progress (eapply rel_exp_Cred; [apply Cred_seq_assoc|]).
-      eapply rel_exp_Cred; [apply Cred_set|].
+      norm_seq; Cstep Cred_set.
       { admit. }
-      eapply rel_exp_Cred; [apply Cred_set|].
+      Cstep Cred_set.
       { admit. }
-      eapply rel_exp_Cred; [eapply Cred_assign|].
+      Cstep Cred_assign.
       (* TODO:
            Want assumption like
              state_ok env tenv m
@@ -1418,7 +1891,7 @@ Proof.
   - (* case x of { ces } *)
     rename v into x, l into ces; cbn.
     bind_step ces' Hces; destruct ces' as [[[boxed_cases unboxed_cases] fvs_cs] n_cs].
-    intros* Hρ; eapply rel_exp_Cred; [eapply Cred_if'|].
+    intros* Hρ; Cstep' Cred_if.
     { admit. }
     { admit. }
     revert boxed_cases unboxed_cases fvs_cs n_cs Hces ρ env tenv m Hρ.
@@ -1438,12 +1911,11 @@ Proof.
     rename v into x, v0 into y; cbn.
     bind_step e' He; destruct e' as [[stm_e fvs_e] n_e].
     intros* Hρ; apply rel_exp_proj; intros* Hy Hproj.
-    eapply rel_exp_Cred; [eapply Cred_set|].
+    Cstep Cred_set.
     { admit. }
     specialize (IHe e); rewrite He in IHe; apply IHe. Guarded.
-    eapply rel_env_antimon_S.
-    { apply (Included_Union_Setminus _ [set x]); eauto with Decidable_DB. }
-    eapply rel_env_antimon_S in Hρ; [|normalize_occurs_free; apply Included_refl].
+    eapply rel_env_antimon_S; [apply (Included_Union_Setminus _ [set x]); sets|].
+    normalize_occurs_free_in Hρ.
     rewrite rel_env_union in Hρ; destruct Hρ as [_ Hρ].
     rewrite rel_env_union; split; [apply rel_env_gso; [intros Hin; now inv Hin|auto] |].
     apply rel_env_gss_sing.
@@ -1452,13 +1924,21 @@ Proof.
     rename v into x, v0 into f, f into ft, l into ys; cbn.
     bind_step e' He; destruct e' as [[stm_e live_after_call] n_e].
     bind_step call Hcall; intros* Hρ.
-    repeat progress (eapply rel_exp_Cred; [apply Cred_seq_assoc|]).
-    admit. (* TODO: proof sketch *)
+    norm_seq.
+    admit.
+    (* idea: we get from the call that the values in the shadow stack are preserved.
+       (that is, if stack represents vs before call then stack still represents vs after call.)
+       this includes all of the variables live after the call (except x, which isn't defined yet)
+       we then push x onto the shadow stack, and maybe call gc.
+       gc spec will say that all the values on the shadow stack are preserved.
+       this includes, again, all the variables live after the call.
+       thus ρ is still related to the heap wrt fvs(e) and we can instantiate IHe accordingly *)
   - (* let rec fds in e *) exact I.
   - (* f ft ys *)
     rename v into f, f into ft, l into ys; cbn.
     bind_step call Hcall; intros* Hρ.
-    apply rel_exp_app; intros* Hfun Hget_ys Hfind_def Hset_lists.
+    apply rel_exp_app; intros* -> Hfun Hget_ys Hfind_def Hset_lists.
+    (* TODO: lemma about make_fun_call *)
     admit.
   - (* let x = Prim p ys in e *)
     rename v into x, l into ys; cbn.
@@ -1466,7 +1946,25 @@ Proof.
     intros* Hρ; apply rel_exp_prim.
   - (* halt x *)
     rename v into x; cbn; intros* Hρ.
-    eapply rel_exp_Cred; [apply Cred_seq_assoc|].
+    norm_seq; Cstep Cred_assign.
+    { admit. }
+    { admit. }
+    { admit. }
+    { admit. }
+    Cstep Cred_assign.
+    { admit. }
+    { admit. }
+    { admit. }
+    { admit. }
+    Cstep' Cred_assign.
+    { admit. }
+    { admit. }
+    { admit. }
+    { admit. }
+    (* TODO: lemma rel_exp_halt
+                ρ(x) ~ᵥ{k} (m, args[1])
+         ---------------------------------------
+         (ρ, Ehalt x) ~{k} (env, tenv, m, Sskip) *)
     admit.
 Abort.
 
